Version MoSel

cfrontend/SimplExprproof.v
@@ -11,765 +11,643 @@
 (* *********************************************************************)
 
 (** Correctness proof for expression simplification. *)
-
 Require Import FunInd.
-Require Import Coqlib Maps Errors Integers.
+Require Import Coqlib (* Maps *) Errors Integers.
+Require Import MoSel Locally SimplExpr SimplExprspec.
 Require Import AST Linking.
 Require Import Values Memory Events Globalenvs Smallstep.
 Require Import Ctypes Cop Csyntax Csem Cstrategy Clight.
-Require Import SimplExpr SimplExprspec.
+Import Maps.PTree.
 
+Local Open Scope gensym_monad_scope.
+Notation "a ! b" := (get b a) (at level 1).
 (** ** Relational specification of the translation. *)
 
 Definition match_prog (p: Csyntax.program) (tp: Clight.program) :=
-    match_program (fun ctx f tf => tr_fundef f tf) eq p tp
- /\ prog_types tp = prog_types p.
+  match_program (fun ctx f tf => tr_fundef f tf) eq p tp
+  /\ prog_types tp = prog_types p.
 
 Lemma transf_program_match:
   forall p tp, transl_program p = OK tp -> match_prog p tp.
 Proof.
   unfold transl_program; intros. monadInv H. split; auto.
   unfold program_of_program; simpl. destruct x; simpl.
-  eapply match_transform_partial_program_contextual. eexact EQ. 
-  intros. apply transl_fundef_spec; auto. 
+  eapply match_transform_partial_program_contextual. eexact EQ.
+  intros. apply transl_fundef_spec; auto.
 Qed.
 
 (** ** Semantic preservation *)
 
 Section PRESERVATION.
 
-Variable prog: Csyntax.program.
-Variable tprog: Clight.program.
-Hypothesis TRANSL: match_prog prog tprog.
+  Variable prog: Csyntax.program.
+  Variable tprog: Clight.program.
+  Hypothesis TRANSL: match_prog prog tprog.
 
-Let ge := Csem.globalenv prog.
-Let tge := Clight.globalenv tprog.
+  Let ge := Csem.globalenv prog.
+  Let tge := Clight.globalenv tprog.
 
-(** Invariance properties. *)
+  (** Invariance properties. *)
 
-Lemma comp_env_preserved:
-  Clight.genv_cenv tge = Csem.genv_cenv ge.
-Proof.
-  simpl. destruct TRANSL. generalize (prog_comp_env_eq tprog) (prog_comp_env_eq prog). 
-  congruence.
-Qed.
+  Lemma comp_env_preserved:
+    Clight.genv_cenv tge = Csem.genv_cenv ge.
+  Proof.
+    simpl. destruct TRANSL. generalize (prog_comp_env_eq tprog) (prog_comp_env_eq prog).
+    congruence.
+  Qed.
 
-Lemma symbols_preserved:
-  forall (s: ident), Genv.find_symbol tge s = Genv.find_symbol ge s.
-Proof (Genv.find_symbol_match (proj1 TRANSL)).
+  Lemma symbols_preserved:
+    forall (s: ident), Genv.find_symbol tge s = Genv.find_symbol ge s.
+  Proof (Genv.find_symbol_match (proj1 TRANSL)).
 
-Lemma senv_preserved:
-  Senv.equiv ge tge.
-Proof (Genv.senv_match (proj1 TRANSL)).
+  Lemma senv_preserved:
+    Senv.equiv ge tge.
+  Proof (Genv.senv_match (proj1 TRANSL)).
 
-Lemma function_ptr_translated:
-  forall b f,
-  Genv.find_funct_ptr ge b = Some f ->
-  exists tf,
-  Genv.find_funct_ptr tge b = Some tf /\ tr_fundef f tf.
-Proof.
-  intros.
-  edestruct (Genv.find_funct_ptr_match (proj1 TRANSL)) as (ctx & tf & A & B & C); eauto.
-Qed.
+  Lemma function_ptr_translated:
+    forall b f,
+      Genv.find_funct_ptr ge b = Some f ->
+      exists tf,
+        Genv.find_funct_ptr tge b = Some tf /\ tr_fundef f tf.
+  Proof.
+    intros.
+    edestruct (Genv.find_funct_ptr_match (proj1 TRANSL)) as (ctx & tf & A & B & C); eauto.
+  Qed.
 
-Lemma functions_translated:
-  forall v f,
-  Genv.find_funct ge v = Some f ->
-  exists tf,
-  Genv.find_funct tge v = Some tf /\ tr_fundef f tf.
-Proof.
-  intros.
-  edestruct (Genv.find_funct_match (proj1 TRANSL)) as (ctx & tf & A & B & C); eauto.
-Qed.
+  Lemma functions_translated:
+    forall v f,
+      Genv.find_funct ge v = Some f ->
+      exists tf,
+        Genv.find_funct tge v = Some tf /\ tr_fundef f tf.
+  Proof.
+    intros.
+    edestruct (Genv.find_funct_match (proj1 TRANSL)) as (ctx & tf & A & B & C); eauto.
+  Qed.
 
-Lemma type_of_fundef_preserved:
-  forall f tf, tr_fundef f tf ->
-  type_of_fundef tf = Csyntax.type_of_fundef f.
-Proof.
-  intros. inv H.
-  inv H0; simpl. unfold type_of_function, Csyntax.type_of_function. congruence.
-  auto.
-Qed.
+  Lemma type_of_fundef_preserved:
+    forall f tf, tr_fundef f tf ->
+            type_of_fundef tf = Csyntax.type_of_fundef f.
+  Proof.
+    intros. inv H.
+    inv H0; simpl. unfold type_of_function, Csyntax.type_of_function. congruence.
+    auto.
+  Qed.
 
-Lemma function_return_preserved:
-  forall f tf, tr_function f tf ->
-  fn_return tf = Csyntax.fn_return f.
-Proof.
-  intros. inv H; auto.
-Qed.
+  Lemma function_return_preserved:
+    forall f tf, tr_function f tf ->
+            fn_return tf = Csyntax.fn_return f.
+  Proof.
+    intros. inv H; auto.
+  Qed.
 
-(** Properties of smart constructors. *)
+  (** Properties of smart constructors. *)
 
-Lemma eval_Ederef':
-  forall ge e le m a t l ofs,
-  eval_expr ge e le m a (Vptr l ofs) ->
-  eval_lvalue ge e le m (Ederef' a t) l ofs.
-Proof.
-  intros. unfold Ederef'; destruct a; auto using eval_Ederef.
-  destruct (type_eq t (typeof a)); auto using eval_Ederef.
-  inv H.
-- auto. 
-- inv H0.
-Qed.
+  Lemma eval_Ederef':
+    forall ge e le m a t l ofs,
+      eval_expr ge e le m a (Vptr l ofs) ->
+      eval_lvalue ge e le m (Ederef' a t) l ofs.
+  Proof.
+    intros. unfold Ederef'; destruct a; auto using eval_Ederef.
+    destruct (type_eq t0 (typeof a)); auto using eval_Ederef.
+    inv H.
+    - auto.
+    - inv H0.
+  Qed.
 
-Lemma typeof_Ederef':
-  forall a t, typeof (Ederef' a t) = t.
-Proof.
-  unfold Ederef'; intros; destruct a; auto. destruct (type_eq t (typeof a)); auto. 
-Qed.
+  Lemma typeof_Ederef':
+    forall a t, typeof (Ederef' a t) = t.
+  Proof.
+    unfold Ederef'; intros; destruct a; auto. destruct (type_eq t0 (typeof a)); auto.
+  Qed.
 
-Lemma eval_Eaddrof':
-  forall ge e le m a t l ofs,
-  eval_lvalue ge e le m a l ofs ->
-  eval_expr ge e le m (Eaddrof' a t) (Vptr l ofs).
-Proof.
-  intros. unfold Eaddrof'; destruct a; auto using eval_Eaddrof.
-  destruct (type_eq t (typeof a)); auto using eval_Eaddrof.
-  inv H; auto.
-Qed.
+  Lemma eval_Eaddrof':
+    forall ge e le m a t l ofs,
+      eval_lvalue ge e le m a l ofs ->
+      eval_expr ge e le m (Eaddrof' a t) (Vptr l ofs).
+  Proof.
+    intros. unfold Eaddrof'; destruct a; auto using eval_Eaddrof.
+    destruct (type_eq t0 (typeof a)); auto using eval_Eaddrof.
+    inv H; auto.
+  Qed.
 
-Lemma typeof_Eaddrof':
-  forall a t, typeof (Eaddrof' a t) = t.
-Proof.
-  unfold Eaddrof'; intros; destruct a; auto. destruct (type_eq t (typeof a)); auto. 
-Qed.
+  Lemma typeof_Eaddrof':
+    forall a t, typeof (Eaddrof' a t) = t.
+  Proof.
+    unfold Eaddrof'; intros; destruct a; auto. destruct (type_eq t0 (typeof a)); auto.
+  Qed.
 
-(** Translation of simple expressions. *)
+  (** Translation of simple expressions. *)
 
-Lemma tr_simple_nil:
-  (forall le dst r sl a tmps, tr_expr le dst r sl a tmps ->
-   dst = For_val \/ dst = For_effects -> simple r = true -> sl = nil)
-/\(forall le rl sl al tmps, tr_exprlist le rl sl al tmps ->
-   simplelist rl = true -> sl = nil).
-Proof.
-  assert (A: forall dst a, dst = For_val \/ dst = For_effects -> final dst a = nil).
-    intros. destruct H; subst dst; auto.
-  apply tr_expr_exprlist; intros; simpl in *; try discriminate; auto.
-- rewrite H0; auto. simpl; auto.
-- rewrite H0; auto. simpl; auto.
-- destruct H1; congruence.
-- destruct (andb_prop _ _ H6). inv H1.
-    rewrite H0; eauto. simpl; auto.
-    unfold chunk_for_volatile_type in H9.
-    destruct (type_is_volatile (Csyntax.typeof e1)); simpl in H8; congruence.
-- rewrite H0; auto. simpl; auto.
-- rewrite H0; auto. simpl; auto.
-- destruct (andb_prop _ _ H7). rewrite H0; auto. rewrite H2; auto. simpl; auto.
-- rewrite H0; auto. simpl; auto.
-- destruct (andb_prop _ _ H6). rewrite H0; auto.
-Qed.
+  Lemma pair_equal_spec :
+    forall (A B : Type) (a1 a2 : A) (b1 b2 : B),
+      (a1, b1) = (a2, b2) <-> a1 = a2 /\ b1 = b2.
+  Proof.
+    intros. split; intro H; inversion H; subst; eauto.
+  Qed.
 
-Lemma tr_simple_expr_nil:
-  forall le dst r sl a tmps, tr_expr le dst r sl a tmps ->
-  dst = For_val \/ dst = For_effects -> simple r = true -> sl = nil.
-Proof (proj1 tr_simple_nil).
+  Import adequacy.
 
-Lemma tr_simple_exprlist_nil:
-  forall le rl sl al tmps, tr_exprlist le rl sl al tmps ->
-  simplelist rl = true -> sl = nil.
-Proof (proj2 tr_simple_nil).
+  Local Set Warnings "-deprecated".
 
-(** Translation of [deref_loc] and [assign_loc] operations. *)
+  Ltac apply_ind_simple_nil l h :=
+    match goal with
+    | H : Datatypes.negb _ = true |- _ => apply negb_true_iff in H; apply_ind_simple_nil l h
+    | H :  _ && _ = true |- _ =>
+      let P0 := fresh "P" in
+      let P1 := fresh "P" in
+      apply andb_true_iff in H as (P0&P1); apply_ind_simple_nil l h
+    | H : forall _ _ _ _, bi_emp_valid (tr_expr _ _ l _ _ -∗ _)
+                     |- _ => iDestruct (H with h) as h; iDestruct (h with "[] []") as "%"; auto
+    | H : forall _ _ _ , bi_emp_valid (tr_exprlist _ l _ _ -∗ _)
+                    |- _ => iDestruct (H with h) as h; iDestruct (h with "[]") as "%"; auto
+    | _ => idtac
+    end.
 
-Remark deref_loc_translated:
-  forall ty m b ofs t v,
-  Csem.deref_loc ge ty m b ofs t v ->
-  match chunk_for_volatile_type ty with
-  | None => t = E0 /\ Clight.deref_loc ty m b ofs v
-  | Some chunk => volatile_load tge chunk m b ofs t v
-  end.
-Proof.
-  intros. unfold chunk_for_volatile_type. inv H.
-  (* By_value, not volatile *)
-  rewrite H1. split; auto. eapply deref_loc_value; eauto.
-  (* By_value, volatile *)
-  rewrite H0; rewrite H1. eapply volatile_load_preserved with (ge1 := ge); auto. apply senv_preserved.
-  (* By reference *)
-  rewrite H0. destruct (type_is_volatile ty); split; auto; eapply deref_loc_reference; eauto.
-  (* By copy *)
-  rewrite H0. destruct (type_is_volatile ty); split; auto; eapply deref_loc_copy; eauto.
-Qed.
+  Ltac apply_ind_core f list_ident :=
+    match list_ident with
+    | [] => idtac
+    | ?h :: ?t =>
+      let env := iGetCtx in
+      let P := reduction.pm_eval (envs_lookup h env) in
+      match P with
+      | Some (false, ?P) =>
+        match P with
+        | tr_expr _ _ ?l _ _ => f l h; apply_ind_core f t
+        | tr_exprlist _ ?l _ _ => f l h; apply_ind_core f t
+        | tr_rvalof _ ?l _ _ => f l h; apply_ind_core f t
+        | _ => apply_ind_core f t
+        end
+      | _ => idtac
+      end
+    | _ => idtac
+    end.
 
-Remark assign_loc_translated:
-  forall ty m b ofs v t m',
-  Csem.assign_loc ge ty m b ofs v t m' ->
-  match chunk_for_volatile_type ty with
-  | None => t = E0 /\ Clight.assign_loc tge ty m b ofs v m'
-  | Some chunk => volatile_store tge chunk m b ofs v t m'
-  end.
-Proof.
-  intros. unfold chunk_for_volatile_type. inv H.
-  (* By_value, not volatile *)
-  rewrite H1. split; auto. eapply assign_loc_value; eauto.
-  (* By_value, volatile *)
-  rewrite H0; rewrite H1. eapply volatile_store_preserved with (ge1 := ge); auto. apply senv_preserved.
-  (* By copy *)
-  rewrite H0. rewrite <- comp_env_preserved in *.
-  destruct (type_is_volatile ty); split; auto; eapply assign_loc_copy; eauto.
-Qed.
+  Ltac apply_ind f :=
+    iStartProof;
+    let env := iGetCtx in
+    let list_ident := eval compute in (rev (envs_dom env)) in
+        apply_ind_core f list_ident.
 
-(** Evaluation of simple expressions and of their translation *)
+  Lemma tr_simple_nil:
+    (forall r dst sl le a,
+        ⊢ tr_expr le dst r sl a -∗
+          ⌜ dst = For_val \/ dst = For_effects ⌝ -∗
+                                              ⌜ simple r = true ⌝ -∗
+                                                                ⌜sl = nil ⌝)
+    /\(forall rl le sl al, ⊢ tr_exprlist le rl sl al -∗ ⌜ simplelist rl = true ⌝ -∗ ⌜ sl = nil ⌝).
+  Proof.
+    apply tr_expr_exprlist; intros; simpl in *; try discriminate; auto;
+      iIntros; norm_all; apply_ind apply_ind_simple_nil; try(destruct a0; subst; norm_all).
+    - unfold tr_rvalof; rewrite P0; norm_all; subst; auto.
+    - unfold tr_rvalof; rewrite P0; norm_all; subst; auto.
+    - destruct a; auto.
+    - subst; auto.
+  Qed.
 
-Lemma tr_simple:
- forall e m,
- (forall r v,
-  eval_simple_rvalue ge e m r v ->
-  forall le dst sl a tmps,
-  tr_expr le dst r sl a tmps ->
-  match dst with
-  | For_val => sl = nil /\ Csyntax.typeof r = typeof a /\ eval_expr tge e le m a v
-  | For_effects => sl = nil
-  | For_set sd =>
-      exists b, sl = do_set sd b
-             /\ Csyntax.typeof r = typeof b
-             /\ eval_expr tge e le m b v
-  end)
-/\
- (forall l b ofs,
-  eval_simple_lvalue ge e m l b ofs ->
-  forall le sl a tmps,
-  tr_expr le For_val l sl a tmps ->
-  sl = nil /\ Csyntax.typeof l = typeof a /\ eval_lvalue tge e le m a b ofs).
-Proof.
-Opaque makeif.
-  intros e m.
-  apply (eval_simple_rvalue_lvalue_ind ge e m); intros until tmps; intros TR; inv TR.
-- (* value *)
-  auto.
-- auto.
-- exists a0; auto.
-- (* rvalof *)
-  inv H7; try congruence.
-  exploit H0; eauto. intros [A [B C]].
-  subst sl1; simpl.
-  assert (eval_expr tge e le m a v).
-    eapply eval_Elvalue. eauto.
-    rewrite <- B.
-    exploit deref_loc_translated; eauto. unfold chunk_for_volatile_type; rewrite H2. tauto.
-  destruct dst; auto.
-  econstructor. split. simpl; eauto. auto.
-- (* addrof *)
-  exploit H0; eauto. intros [A [B C]].
-  subst sl1; simpl.
-  assert (eval_expr tge e le m (Eaddrof' a1 ty) (Vptr b ofs)) by (apply eval_Eaddrof'; auto).
-  assert (typeof (Eaddrof' a1 ty) = ty) by (apply typeof_Eaddrof').
-  destruct dst; auto. simpl; econstructor; eauto.  
-- (* unop *)
-  exploit H0; eauto. intros [A [B C]].
-  subst sl1; simpl.
-  assert (eval_expr tge e le m (Eunop op a1 ty) v). econstructor; eauto. congruence.
-  destruct dst; auto. simpl; econstructor; eauto.
-- (* binop *)
-  exploit H0; eauto. intros [A [B C]].
-  exploit H2; eauto. intros [D [E F]].
-  subst sl1 sl2; simpl.
-  assert (eval_expr tge e le m (Ebinop op a1 a2 ty) v). econstructor; eauto. rewrite comp_env_preserved; congruence.
-  destruct dst; auto. simpl; econstructor; eauto.
-- (* cast effects *)
-  exploit H0; eauto.
-- (* cast val *)
-  exploit H0; eauto. intros [A [B C]].
-  subst sl1; simpl.
-  assert (eval_expr tge e le m (Ecast a1 ty) v). econstructor; eauto. congruence.
-  destruct dst; auto. simpl; econstructor; eauto.
-- (* sizeof *)
-  rewrite <- comp_env_preserved.
-  destruct dst.
-  split; auto. split; auto. constructor.
-  auto.
-  exists (Esizeof ty1 ty). split. auto. split. auto. constructor.
-- (* alignof *)
-  rewrite <- comp_env_preserved.
-  destruct dst.
-  split; auto. split; auto. constructor.
-  auto.
-  exists (Ealignof ty1 ty). split. auto. split. auto. constructor.
-- (* var local *)
-  split; auto. split; auto. apply eval_Evar_local; auto.
-- (* var global *)
-  split; auto. split; auto. apply eval_Evar_global; auto.
-    rewrite symbols_preserved; auto.
-- (* deref *)
-  exploit H0; eauto. intros [A [B C]]. subst sl1.
-  split; auto. split. rewrite typeof_Ederef'; auto. apply eval_Ederef'; auto. 
-- (* field struct *)
-  rewrite <- comp_env_preserved in *.
-  exploit H0; eauto. intros [A [B C]]. subst sl1.
-  split; auto. split; auto. rewrite B in H1. eapply eval_Efield_struct; eauto.
-- (* field union *)
-  rewrite <- comp_env_preserved in *.
-  exploit H0; eauto. intros [A [B C]]. subst sl1.
-  split; auto. split; auto. rewrite B in H1. eapply eval_Efield_union; eauto.
-Qed.
+  Lemma tr_simple_expr_nil:
+    (forall r dst sl le a,
+        ⊢ tr_expr le dst r sl a -∗
+        ⌜ dst = For_val \/ dst = For_effects ⌝ -∗
+        ⌜ simple r = true ⌝ -∗
+        ⌜sl = nil ⌝).
+  Proof. apply (proj1 tr_simple_nil). Qed.
 
-Lemma tr_simple_rvalue:
-  forall e m r v,
-  eval_simple_rvalue ge e m r v ->
-  forall le dst sl a tmps,
-  tr_expr le dst r sl a tmps ->
-  match dst with
-  | For_val => sl = nil /\ Csyntax.typeof r = typeof a /\ eval_expr tge e le m a v
-  | For_effects => sl = nil
-  | For_set sd =>
-      exists b, sl = do_set sd b
-             /\ Csyntax.typeof r = typeof b
-             /\ eval_expr tge e le m b v
-  end.
-Proof.
-  intros e m. exact (proj1 (tr_simple e m)).
-Qed.
+  Lemma tr_simple_exprlist_nil:
+    (forall rl le sl al, ⊢ tr_exprlist le rl sl al -∗
+                      ⌜ simplelist rl = true ⌝ -∗ ⌜ sl = nil ⌝).
+  Proof. apply (proj2 tr_simple_nil). Qed.
 
-Lemma tr_simple_lvalue:
-  forall e m l b ofs,
-  eval_simple_lvalue ge e m l b ofs ->
-  forall le sl a tmps,
-  tr_expr le For_val l sl a tmps ->
-  sl = nil /\ Csyntax.typeof l = typeof a /\ eval_lvalue tge e le m a b ofs.
-Proof.
-  intros e m. exact (proj2 (tr_simple e m)).
-Qed.
 
-Lemma tr_simple_exprlist:
-  forall le rl sl al tmps,
-  tr_exprlist le rl sl al tmps ->
-  forall e m tyl vl,
-  eval_simple_list ge e m rl tyl vl ->
-  sl = nil /\ eval_exprlist tge e le m al tyl vl.
-Proof.
-  induction 1; intros.
-  inv H. split. auto. constructor.
-  inv H4.
-  exploit tr_simple_rvalue; eauto. intros [A [B C]].
-  exploit IHtr_exprlist; eauto. intros [D E].
-  split. subst; auto. econstructor; eauto. congruence.
-Qed.
+  (** Translation of [deref_loc] and [assign_loc] operations. *)
 
-(** Commutation between the translation of expressions and left contexts. *)
+  Remark deref_loc_translated:
+    forall ty m b ofs t v,
+      Csem.deref_loc ge ty m b ofs t v ->
+      match chunk_for_volatile_type ty with
+      | None => t = E0 /\ Clight.deref_loc ty m b ofs v
+      | Some chunk => volatile_load tge chunk m b ofs t v
+      end.
+  Proof.
+    intros. unfold chunk_for_volatile_type. inv H.
+    (* By_value, not volatile *)
+    rewrite H1. split; auto. eapply deref_loc_value; eauto.
+    (* By_value, volatile *)
+    rewrite H0; rewrite H1. eapply volatile_load_preserved with (ge1 := ge); auto. apply senv_preserved.
+    (* By reference *)
+    rewrite H0. destruct (type_is_volatile ty); split; auto; eapply deref_loc_reference; eauto.
+    (* By copy *)
+    rewrite H0. destruct (type_is_volatile ty); split; auto; eapply deref_loc_copy; eauto.
+  Qed.
 
-Lemma typeof_context:
-  forall k1 k2 C, leftcontext k1 k2 C ->
-  forall e1 e2, Csyntax.typeof e1 = Csyntax.typeof e2 ->
-  Csyntax.typeof (C e1) = Csyntax.typeof (C e2).
-Proof.
-  induction 1; intros; auto.
-Qed.
+  Remark assign_loc_translated:
+    forall ty m b ofs v t m',
+      Csem.assign_loc ge ty m b ofs v t m' ->
+      match chunk_for_volatile_type ty with
+      | None => t = E0 /\ Clight.assign_loc tge ty m b ofs v m'
+      | Some chunk => volatile_store tge chunk m b ofs v t m'
+      end.
+  Proof.
+    intros. unfold chunk_for_volatile_type. inv H.
+    (* By_value, not volatile *)
+    rewrite H1. split; auto. eapply assign_loc_value; eauto.
+    (* By_value, volatile *)
+    rewrite H0; rewrite H1. eapply volatile_store_preserved with (ge1 := ge); auto. apply senv_preserved.
+    (* By copy *)
+    rewrite H0. rewrite <- comp_env_preserved in *.
+    destruct (type_is_volatile ty); split; auto; eapply assign_loc_copy; eauto.
+  Qed.
+
+  Ltac apply_ind_simple l h :=
+    match goal with
+    | H : forall _ _ _, bi_emp_valid (tr_expr _ _ l _ _ -∗ _) |- _ =>
+      iDestruct (H with h) as "[% [% %]]"; iClear h
+    | H : forall _ _ _ _, bi_emp_valid (tr_expr _ _ l _ _ -∗ _) |- _ =>
+      iDestruct (H with h) as "[% [% %]]"; iClear h
+    | _ => fail "No rec"
+    end.
+
+  (** Evaluation of simple expressions and of their translation *)
+  Lemma tr_simple:
+    forall e m,
+      (forall r v,
+          eval_simple_rvalue ge e m r v ->
+          forall le dst sl a,
+            ⊢ tr_expr le dst r sl a -∗
+              ⌜ match dst with
+                | For_val => sl = nil /\ Csyntax.typeof r = typeof a /\ eval_expr tge e le m a v
+                | For_effects => sl = nil
+                | For_set sd =>
+                  exists b, sl = do_set sd b /\ Csyntax.typeof r = typeof b /\ eval_expr tge e le m b v
+                end⌝)
+      /\
+      (forall l b ofs,
+          eval_simple_lvalue ge e m l b ofs ->
+          forall le sl a, ⊢ tr_expr le For_val l sl a -∗
+                       ⌜ sl = nil /\ Csyntax.typeof l = typeof a /\ eval_lvalue tge e le m a b ofs ⌝).
+  Proof.
+    Opaque makeif.
+    intros e m.
+    apply (eval_simple_rvalue_lvalue_ind ge e m); intros; simpl; iIntros; norm_all;
+      apply_ind apply_ind_simple.
+    (* value *)
+    - destruct dst; simpl in *; norm_all.
+      + repeat (iSplit; auto). iDestruct (locally_elim with "HD") as "HA". iFrame.
+      + iDestruct "HB" as "[_ HA]". norm_all. repeat iExists _. repeat iSplit; auto.
+        iDestruct (locally_elim with "HD") as "HA". iFrame.
+    (* rvalof *)
+    - unfold tr_rvalof. subst. rewrite H2. norm_all. subst.
+      destruct dst; simpl; eauto; repeat iExists _; repeat iSplit; auto; iPureIntro; econstructor;
+        eauto; exploit deref_loc_translated; eauto; unfold chunk_for_volatile_type.
+      + rewrite H2. intros [P0 P1]. rewrite <- H6; auto.
+      + rewrite H2. intros [P0 P1]. rewrite <- H6; auto.
+    - destruct dst; simpl in *; subst; auto; repeat iExists _; repeat iSplit; iPureIntro; simpl;
+        auto. rewrite (typeof_Eaddrof' _ ty); auto. eapply eval_Eaddrof'; auto.
+      rewrite (typeof_Eaddrof' _ ty); auto. eapply eval_Eaddrof'; auto.
+    - destruct dst; simpl in *; subst; auto; repeat iExists _; repeat iSplit; iPureIntro; simpl;
+        auto; econstructor; eauto; rewrite <- H5; auto.
+    - rewrite <- comp_env_preserved in H3.
+      subst. iPureIntro. rewrite H7 in H3. rewrite H10 in H3.
+      destruct dst; simpl; simpl_list; auto.
+      + repeat split; auto. econstructor; eauto.
+      + eexists. repeat split; auto. econstructor; eauto.
+    - subst. iPureIntro. rewrite H5 in H1. destruct dst; simpl in *; auto.
+      + repeat split; auto. econstructor; eauto.
+      + eexists. repeat split; eauto. econstructor; eauto.
+    - iPureIntro. subst.
+      destruct dst; simpl in *; simpl_list; auto; repeat eexists; pose (P := comp_env_preserved);
+        simpl in P; rewrite <- P; apply eval_Esizeof.
+    - iPureIntro. subst. destruct dst; simpl in *; auto; repeat eexists; repeat split; auto;
+                           pose (P := comp_env_preserved); simpl in P; rewrite <- P; constructor.
+    - iStopProof. iIntros "#>[_ [% %]]". iPureIntro. subst. repeat split; auto. constructor. apply H.
+    - iStopProof. iIntros "#>[_ [% %]]". iPureIntro. subst. repeat split; auto.
+      apply eval_Evar_global; auto. rewrite symbols_preserved; auto.
+    - subst. iPureIntro. repeat split. rewrite typeof_Ederef'. auto. apply eval_Ederef'; auto.
+    - subst. iPureIntro. repeat split. rewrite <- comp_env_preserved in *.
+      eapply eval_Efield_struct; eauto. rewrite <- H7. eauto.
+    - subst. iPureIntro. repeat split; auto. rewrite <- comp_env_preserved in *. rewrite H6 in H1.
+      eapply eval_Efield_union; eauto.
+  Qed.
+
+  Lemma tr_simple_rvalue:
+    forall e m r v,
+      eval_simple_rvalue ge e m r v ->
+      forall le dst sl a,
+        ⊢ tr_expr le dst r sl a -∗
+          ⌜ match dst with
+            | For_val => sl = nil /\ Csyntax.typeof r = typeof a /\ eval_expr tge e le m a v
+            | For_effects => sl = nil
+            | For_set sd =>
+              exists b, sl = do_set sd b /\ Csyntax.typeof r = typeof b /\ eval_expr tge e le m b v
+            end⌝.
+  Proof.
+    intros e m. exact (proj1 (tr_simple e m)).
+  Qed.
+
+  Lemma tr_simple_lvalue:
+    forall e m l b ofs,
+      eval_simple_lvalue ge e m l b ofs ->
+      forall le sl a, ⊢ tr_expr le For_val l sl a -∗
+                   ⌜ sl = nil /\ Csyntax.typeof l = typeof a /\ eval_lvalue tge e le m a b ofs ⌝.
+  Proof.
+    intros e m. exact (proj2 (tr_simple e m)).
+  Qed.
+
+  Lemma tr_simple_exprlist:
+    forall le rl sl al,
+      ⊢ tr_exprlist le rl sl al -∗
+        ∀ e m tyl vl,
+          ⌜ eval_simple_list ge e m rl tyl vl ⌝ -∗
+            ⌜ sl = nil /\ eval_exprlist tge e le m al tyl vl ⌝.
+  Proof.
+    induction rl.
+    - iIntros. inversion a.
+      iPureIntro. repeat split; eauto. inversion a0. subst. constructor.
+    - simpl. iIntros. norm_all. inversion a. subst. iDestruct (IHrl with "HD []") as "[% %]"; eauto.
+      iDestruct (tr_simple_rvalue with "HB") as "[% [% %]]"; eauto.
+      iPureIntro. subst. split; auto. econstructor; eauto. rewrite <- H2. eauto.
+  Qed.
+
+  (** Commutation between the translation of expressions and left contexts. *)
+
+  Lemma typeof_context:
+    forall k1 k2 C, leftcontext k1 k2 C ->
+               forall e1 e2, Csyntax.typeof e1 = Csyntax.typeof e2 ->
+                        Csyntax.typeof (C e1) = Csyntax.typeof (C e2).
+  Proof.
+    induction 1; intros; auto.
+  Qed.
+
+
+  Ltac apply_ind_invariant l h :=
+    match goal with
+    | H : forall _ _ _ _, bi_emp_valid (tr_expr _ _ l _ _ -∗ _) |- _ =>
+      iDestruct (H with h) as h
+    | H : forall _ _ _, bi_emp_valid (tr_exprlist _ l _ _ -∗ _) |- _ =>
+      iDestruct (H with h) as h
+    | _ => fail "No rec"
+    end.
+
+  Ltac locally_core b :=
+    match goal with
+    | |- envs_entails _ (locally ?le (fun le' => ∀ a, ?P )) =>
+      iApply locally_forall; iIntros "*"; locally_core b
+    | |- envs_entails _ (locally ?le (fun le' => ∃ a , ?P )) =>
+      match b with
+      | true => iApply locally_exists; locally_core b
+      | false => iApply locally_exists'; locally_core b
+      end
+    | |- envs_entails _ (locally ?le (fun le' => locally le' (fun le'' => ?P ))) =>
+      iApply locally_idempotence
+    | |- envs_entails _ (locally ?le (fun _ => ?P )) =>
+      iApply locally_simpl; auto
+    | _ => auto
+    end.
+
+  Lemma tr_expr_invariant :
+    (forall r dst sl a le, ⊢ tr_expr le dst r sl a -∗ locally le (fun le' => tr_expr le' dst r sl a))
+    /\
+    (forall rl le sl al, ⊢ tr_exprlist le rl sl al -∗ locally le (fun le' => tr_exprlist le' rl sl al)).
+  Proof.
+    apply tr_expr_exprlist; intros; iIntros; simpl;
+      try iApply locally_modout; norm_all; try iModIntro; apply_ind apply_ind_invariant;
+        locally_core true.
+    - destruct dst; norm_all; locally_core false.
+      + iApply locally_frame_r; locally_core true; auto.
+      + iApply locally_and. iSplit; locally_core false.
+        * iDestruct "HC" as "[$ _]". auto.
+        * iDestruct "HC" as "[_ HA]". norm_all. iExists _. iApply locally_sep_indep_r.
+        iSplitL "HG"; eauto. locally_core true. eauto. iSplit; auto.
+    - iApply (locally_frame_l with "HE"). locally_core true.
+      iApply locally_sep_indep_r. iSplitL; auto.
+    - iApply (locally_frame_l with "HE"). locally_core true. iApply locally_sep_indep_r.
+      iSplitL "HG"; auto.
+    - iApply (locally_frame_l with "HE"). locally_core true.
+      iApply locally_sep_indep_r. iSplitL; auto.
+    - iApply (locally_frame_l with "HE"). locally_core true. iApply locally_sep_indep_r.
+      iSplitL; auto.
+    - iApply (locally_frame_l with "HE"). locally_core true. iApply locally_sep_indep_r.
+      iSplitL; auto.
+    - iApply (locally_frame_l with "HE"). locally_core true.
+      iApply (locally_delete_2 with "HG HI"). iIntros. iFrame. auto.
+    - iApply (locally_frame_l with "HE"). locally_core true.
+      iApply locally_sep_indep_r. iSplitL; auto.
+    - destruct dst; norm_all; apply_ind apply_ind_invariant; locally_core true;
+      iApply (locally_delete_2 with "HE HG"); iIntros; iFrame; auto.
+    - destruct dst; norm_all; apply_ind apply_ind_invariant; locally_core true;
+        iApply (locally_delete_2 with "HE HG"); iIntros; iFrame; auto.
+    - destruct dst; norm_all; apply_ind apply_ind_invariant; locally_core true.
+      + iApply (locally_sep with "HE"). iApply locally_sep_indep_r.
+        iSplitL; auto. iApply locally_and. iSplit. iDestruct "HG" as "[HB _]". iApply (H0 with "HB").
+        iDestruct "HG" as "[_ HB]". iApply (H1 with "HB").
+      + iApply (locally_delete_3 with "HE HG HI"). iIntros. iFrame. auto.
+      + iApply (locally_frame_l with "HE"). locally_core true.
+        iApply (locally_sep with "HG"). iApply locally_sep_indep_r. iSplitL; auto.
+        iApply locally_and. iSplit. iDestruct "HI" as "[HB _]". iApply (H0 with "HB").
+        iDestruct "HI" as "[_ HB]". iApply (H1 with "HB").
+    - destruct dst; norm_all; apply_ind apply_ind_invariant; locally_core true.
+      + iApply (locally_sep with "HE"). iApply (locally_sep with "HG"). locally_core true.
+      + iApply (locally_delete_2 with "HE HG"). iIntros. iFrame. auto.
+      + iApply (locally_sep with "HE"). iApply (locally_sep with "HG"). locally_core true.
+        iIntros. iSplitL "HI"; auto.
+    - destruct dst; norm_all; apply_ind apply_ind_invariant; locally_core true.
+      + iApply (locally_frame_l with "HE"). locally_core true.
+        iApply (locally_delete_2 with "HG HI"). iIntros. iFrame. auto.
+      + iApply (locally_delete_2 with "HE HG"). iIntros. iFrame. auto.
+      + iApply (locally_frame_l with "HE"). locally_core true.
+        iApply (locally_delete_2 with "HI HG"). iIntros "* $ $". iSplitL "HK"; auto.
+    - destruct dst; norm_all; apply_ind apply_ind_invariant; locally_core true.
+      + iApply (locally_sep with "HE"). iApply (locally_frame_l with "HJ"). locally_core true.
+      + iApply (locally_sep with "HE"). locally_core true.
+      + iApply (locally_sep with "HE"). iApply (locally_frame_l with "HJ"). locally_core true.
+    - iApply (locally_delete_2 with "HE HG"). iIntros "* $ $ //".
+    - destruct dst; norm_all; apply_ind apply_ind_invariant; locally_core true.
+      + iApply (locally_frame_l with "HE"). locally_core true.
+        iApply (locally_delete_2 with "HI HK"). iIntros "* $ $ //". iSplitL; auto.
+      + iApply (locally_delete_2 with "HE HG"). iIntros "* $ $ //".
+      + iApply (locally_frame_l with "HE"). locally_core true.
+        iApply (locally_delete_2 with "HI HK"). iIntros "* $ $ //". iSplitL; auto.
+    - destruct dst; norm_all; apply_ind apply_ind_invariant; locally_core true.
+      + iApply (locally_frame_l with "HE"). locally_core true.
+        iApply (locally_sep with "HG"). locally_core true.
+      + iApply (locally_sep with "HE"). locally_core true.
+      + iApply (locally_frame_l with "HE"). locally_core true.
+        iApply (locally_sep with "HG"). locally_core true.
+    - destruct dst; norm_all; apply_ind apply_ind_invariant; locally_core true.
+      + iApply (locally_sep with "HE"). locally_core true.
+      + instantiate (2 := x0).
+        destruct (Pos.eq_dec x0 (sd_temp sd)); norm_all;
+          apply_ind apply_ind_invariant; locally_core true. iApply locally_sep_indep_r. iFrame.
+    - iApply (locally_delete_2 with "HB HD"). iIntros "* $ $ //".
+  Qed.
+
 
 Scheme leftcontext_ind2 := Minimality for leftcontext Sort Prop
   with leftcontextlist_ind2 := Minimality for leftcontextlist Sort Prop.
 Combined Scheme leftcontext_leftcontextlist_ind from leftcontext_ind2, leftcontextlist_ind2.
 
 Lemma tr_expr_leftcontext_rec:
- (
-  forall from to C, leftcontext from to C ->
-  forall le e dst sl a tmps,
-  tr_expr le dst (C e) sl a tmps ->
-  exists dst', exists sl1, exists sl2, exists a', exists tmp',
-  tr_expr le dst' e sl1 a' tmp'
-  /\ sl = sl1 ++ sl2
-  /\ incl tmp' tmps
-  /\ (forall le' e' sl3,
-        tr_expr le' dst' e' sl3 a' tmp' ->
-        (forall id, ~In id tmp' -> le'!id = le!id) ->
-        Csyntax.typeof e' = Csyntax.typeof e ->
-        tr_expr le' dst (C e') (sl3 ++ sl2) a tmps)
- ) /\ (
-  forall from C, leftcontextlist from C ->
-  forall le e sl a tmps,
-  tr_exprlist le (C e) sl a tmps ->
-  exists dst', exists sl1, exists sl2, exists a', exists tmp',
-  tr_expr le dst' e sl1 a' tmp'
-  /\ sl = sl1 ++ sl2
-  /\ incl tmp' tmps
-  /\ (forall le' e' sl3,
-        tr_expr le' dst' e' sl3 a' tmp' ->
-        (forall id, ~In id tmp' -> le'!id = le!id) ->
-        Csyntax.typeof e' = Csyntax.typeof e ->
-        tr_exprlist le' (C e') (sl3 ++ sl2) a tmps)
-).
+  (forall from to C, leftcontext from to C ->
+  forall le e dst sl a,
+  ⊢ tr_expr le dst (C e) sl a -∗
+  ∃ dst' sl1 sl2 a',
+    tr_expr le dst' e sl1 a'
+    ∗ ⌜ sl = sl1 ++ sl2 ⌝
+    ∗ (∀ e',
+          \⌜ Csyntax.typeof e' = Csyntax.typeof e ⌝ -∗
+       (∀ sl3,
+        locally le (fun le' => tr_expr le' dst' e' sl3 a'
+                              -∗ tr_expr le' dst (C e') (sl3 ++ sl2) a))))
+    /\ (
+    forall from C, leftcontextlist from C ->
+    forall le e sl a,
+    ⊢ tr_exprlist le (C e) sl a -∗
+    ∃ dst' sl1 sl2 a',
+      tr_expr le dst' e sl1 a'
+    ∗ ⌜sl = sl1 ++ sl2⌝
+    ∗ (∀ e',
+    \⌜ Csyntax.typeof e' = Csyntax.typeof e ⌝ -∗
+    (∀ sl3,
+        locally le (fun le' => tr_expr le' dst' e' sl3 a' -∗ tr_exprlist le' (C e') (sl3 ++ sl2) a)))
+    ).
 Proof.
 
-Ltac TR :=
-  econstructor; econstructor; econstructor; econstructor; econstructor;
-  split; [eauto | split; [idtac | split]].
+  Ltac init H0 e' H :=
+    iDestruct (H0 with H) as (dst' sl1 sl0 a') "[HA [% HHHHH]]"; subst;
+    repeat iExists _; iSplitL "HA"; eauto; iSplit;
+    [iPureIntro; simpl; try rewrite <- app_assoc; auto |
+     iIntros "* % *"; iDestruct ("HHHHH" $! e' with "[]") as "HHHHH"; auto;
+     iApply (locally_conseq with "HHHHH"); locally_core true].
 
-Ltac NOTIN :=
-  match goal with
-  | [ H1: In ?x ?l, H2: list_disjoint ?l _ |- ~In ?x _ ] =>
-        red; intro; elim (H2 x x); auto; fail
-  | [ H1: In ?x ?l, H2: list_disjoint _ ?l |- ~In ?x _ ] =>
-        red; intro; elim (H2 x x); auto; fail
-  end.
+  Ltac finish_him := iIntros "**"; try iModIntro; iFrame; repeat iExists _; iFrame;
+                     try rewrite <- app_assoc; auto.
 
-Ltac UNCHANGED :=
-  match goal with
-  | [ H: (forall (id: ident), ~In id _ -> ?le' ! id = ?le ! id) |-
-         (forall (id: ident), In id _ -> ?le' ! id = ?le ! id) ] =>
-      intros; apply H; NOTIN
-  end.
-
-  (*generalize compat_dest_change; intro CDC.*)
-  apply leftcontext_leftcontextlist_ind; intros.
-
-- (* base *)
-  TR. rewrite <- app_nil_end; auto. red; auto.
-  intros. rewrite <- app_nil_end; auto.
-- (* deref *)
-  inv H1.
-  exploit H0; eauto. intros [dst' [sl1' [sl2' [a' [tmp' [P [Q [R S]]]]]]]].
-  TR. subst sl1; rewrite app_ass; eauto. auto.
-  intros. rewrite <- app_ass. econstructor; eauto.
-- (* field *)
-  inv H1.
-  exploit H0. eauto. intros [dst' [sl1' [sl2' [a' [tmp' [P [Q [R S]]]]]]]].
-  TR. subst sl1; rewrite app_ass; eauto. auto.
-  intros. rewrite <- app_ass. econstructor; eauto.
-- (* rvalof *)
-  inv H1.
-  exploit H0; eauto. intros [dst' [sl1' [sl2' [a' [tmp' [P [Q [R S]]]]]]]].
-  TR. subst sl1; rewrite app_ass; eauto. red; eauto.
-  intros. rewrite <- app_ass; econstructor; eauto.
-  exploit typeof_context; eauto. congruence.
-- (* addrof *)
-  inv H1.
-  exploit H0; eauto. intros [dst' [sl1' [sl2' [a' [tmp' [P [Q [R S]]]]]]]].
-  TR. subst sl1; rewrite app_ass; eauto. auto.
-  intros. rewrite <- app_ass. econstructor; eauto.
-- (* unop *)
-  inv H1.
-  exploit H0; eauto. intros [dst' [sl1' [sl2' [a' [tmp' [P [Q [R S]]]]]]]].
-  TR. subst sl1; rewrite app_ass; eauto. auto.
-  intros. rewrite <- app_ass. econstructor; eauto.
-- (* binop left *)
-  inv H1.
-  exploit H0; eauto. intros [dst' [sl1' [sl2' [a' [tmp' [P [Q [R S]]]]]]]].
-  TR. subst sl1. rewrite app_ass. eauto.
-  red; auto.
-  intros. rewrite <- app_ass. econstructor; eauto.
-  eapply tr_expr_invariant; eauto. UNCHANGED.
-- (* binop right *)
-  inv H2.
-  assert (sl1 = nil) by (eapply tr_simple_expr_nil; eauto). subst sl1; simpl.
-  exploit H1; eauto. intros [dst' [sl1' [sl2' [a' [tmp' [P [Q [R S]]]]]]]].
-  TR. subst sl2. rewrite app_ass. eauto.
-  red; auto.
-  intros. rewrite <- app_ass. change (sl3 ++ sl2') with (nil ++ sl3 ++ sl2'). rewrite app_ass. econstructor; eauto.
-  eapply tr_expr_invariant; eauto. UNCHANGED.
-- (* cast *)
-  inv H1.
-+ (* for effects *)
-  exploit H0; eauto. intros [dst' [sl1' [sl2' [a' [tmp' [P [Q [R S]]]]]]]].
-  TR. eauto. auto. 
-  intros. econstructor; eauto.
-+ (* generic *)
-  exploit H0; eauto. intros [dst' [sl1' [sl2' [a' [tmp' [P [Q [R S]]]]]]]].
-  TR. subst sl1. rewrite app_ass. eauto. auto. 
-  intros. rewrite <- app_ass. econstructor; eauto.
-- (* seqand *)
-  inv H1.
-+ (* for val *)
-  exploit H0; eauto. intros [dst' [sl1' [sl2' [a' [tmp' [P [Q [R S]]]]]]]].
-  TR.
-  rewrite Q. rewrite app_ass. eauto.
-  red; auto.
-  intros. rewrite <- app_ass. econstructor. apply S; auto.
-  eapply tr_expr_invariant; eauto. UNCHANGED.
-  auto. auto. auto. auto.
-+ (* for effects *)
-  exploit H0; eauto. intros [dst' [sl1' [sl2' [a' [tmp' [P [Q [R S]]]]]]]].
-  TR.
-  rewrite Q. rewrite app_ass. eauto.
-  red; auto.
-  intros. rewrite <- app_ass. econstructor. apply S; auto.
-  eapply tr_expr_invariant; eauto. UNCHANGED.
-  auto. auto. auto.
-+ (* for set *)
-  exploit H0; eauto. intros [dst' [sl1' [sl2' [a' [tmp' [P [Q [R S]]]]]]]].
-  TR.
-  rewrite Q. rewrite app_ass. eauto.
-  red; auto.
-  intros. rewrite <- app_ass. econstructor. apply S; auto.
-  eapply tr_expr_invariant; eauto. UNCHANGED.
-  auto. auto. auto. auto.
-- (* seqor *)
-  inv H1.
-+ (* for val *)
-  exploit H0; eauto. intros [dst' [sl1' [sl2' [a' [tmp' [P [Q [R S]]]]]]]].
-  TR.
-  rewrite Q. rewrite app_ass. eauto.
-  red; auto.
-  intros. rewrite <- app_ass. econstructor. apply S; auto.
-  eapply tr_expr_invariant; eauto. UNCHANGED.
-  auto. auto. auto. auto.
-+ (* for effects *)
-  exploit H0; eauto. intros [dst' [sl1' [sl2' [a' [tmp' [P [Q [R S]]]]]]]].
-  TR.
-  rewrite Q. rewrite app_ass. eauto.
-  red; auto.
-  intros. rewrite <- app_ass. econstructor. apply S; auto.
-  eapply tr_expr_invariant; eauto. UNCHANGED.
-  auto. auto. auto.
-+ (* for set *)
-  exploit H0; eauto. intros [dst' [sl1' [sl2' [a' [tmp' [P [Q [R S]]]]]]]].
-  TR.
-  rewrite Q. rewrite app_ass. eauto.
-  red; auto.
-  intros. rewrite <- app_ass. econstructor. apply S; auto.
-  eapply tr_expr_invariant; eauto. UNCHANGED.
-  auto. auto. auto. auto.
-- (* condition *)
-  inv H1.
-+ (* for val *)
-  exploit H0; eauto. intros [dst' [sl1' [sl2' [a' [tmp' [P [Q [R S]]]]]]]].
-  TR.
-  rewrite Q. rewrite app_ass. eauto.
-  red; auto.
-  intros. rewrite <- app_ass. econstructor. apply S; auto.
-  eapply tr_expr_invariant; eauto. UNCHANGED.
-  eapply tr_expr_invariant; eauto. UNCHANGED.
-  auto. auto. auto. auto. auto. auto.
-+ (* for effects *)
-  exploit H0; eauto. intros [dst' [sl1' [sl2' [a' [tmp' [P [Q [R S]]]]]]]].
-  TR.
-  rewrite Q. rewrite app_ass. eauto.
-  red; auto.
-  intros. rewrite <- app_ass. eapply tr_condition_effects. apply S; auto.
-  eapply tr_expr_invariant; eauto. UNCHANGED.
-  eapply tr_expr_invariant; eauto. UNCHANGED.
-  auto. auto. auto. auto. auto.
-+ (* for set *)
-  exploit H0; eauto. intros [dst' [sl1' [sl2' [a' [tmp' [P [Q [R S]]]]]]]].
-  TR.
-  rewrite Q. rewrite app_ass. eauto.
-  red; auto.
-  intros. rewrite <- app_ass. eapply tr_condition_set. apply S; auto.
-  eapply tr_expr_invariant; eauto. UNCHANGED.
-  eapply tr_expr_invariant; eauto. UNCHANGED.
-  auto. auto. auto. auto. auto. auto.
-- (* assign left *)
-  inv H1.
-+ (* for effects *)
-  exploit H0; eauto. intros [dst' [sl1' [sl2' [a' [tmp' [P [Q [R S]]]]]]]].
-  TR. subst sl1. rewrite app_ass. eauto.
-  red; auto.
-  intros. rewrite <- app_ass. econstructor. apply S; auto.
-  eapply tr_expr_invariant; eauto. UNCHANGED.
-  auto. auto. auto.
-+ (* for val *)
-  exploit H0; eauto. intros [dst' [sl1' [sl2' [a' [tmp' [P [Q [R S]]]]]]]].
-  TR. subst sl1. rewrite app_ass. eauto.
-  red; auto.
-  intros. rewrite <- app_ass. econstructor. apply S; auto.
-  eapply tr_expr_invariant; eauto. UNCHANGED.
-  auto. auto. auto. auto. auto. auto.
-  eapply typeof_context; eauto.
-  auto.
-- (* assign right *)
-  inv H2.
-+ (* for effects *)
-  assert (sl1 = nil) by (eapply tr_simple_expr_nil; eauto). subst sl1; simpl.
-  exploit H1; eauto. intros [dst' [sl1' [sl2' [a' [tmp' [P [Q [R S]]]]]]]].
-  TR. subst sl2. rewrite app_ass. eauto.
-  red; auto.
-  intros. rewrite <- app_ass. change (sl3 ++ sl2') with (nil ++ (sl3 ++ sl2')). rewrite app_ass.
-  econstructor.
-  eapply tr_expr_invariant; eauto. UNCHANGED.
-  apply S; auto. auto. auto. auto.
-+ (* for val *)
-  assert (sl1 = nil) by (eapply tr_simple_expr_nil; eauto). subst sl1; simpl.
-  exploit H1; eauto. intros [dst' [sl1' [sl2' [a' [tmp' [P [Q [R S]]]]]]]].
-  TR. subst sl2. rewrite app_ass. eauto.
-  red; auto.
-  intros. rewrite <- app_ass. change (sl3 ++ sl2') with (nil ++ (sl3 ++ sl2')). rewrite app_ass.
-  econstructor.
-  eapply tr_expr_invariant; eauto. UNCHANGED.
-  apply S; auto. auto. auto. auto. auto. auto. auto. auto.
-  eapply typeof_context; eauto.
-- (* assignop left *)
-  inv H1.
-+ (* for effects *)
-  exploit H0; eauto. intros [dst' [sl1' [sl2' [a' [tmp' [P [Q [R S]]]]]]]].
-  TR. subst sl1. rewrite app_ass. eauto.
-  red; auto.
-  intros. rewrite <- app_ass. econstructor. apply S; auto.
-  eapply tr_expr_invariant; eauto. UNCHANGED.
-  symmetry; eapply typeof_context; eauto. eauto.
-  auto. auto. auto. auto. auto. auto.
-+ (* for val *)
-  exploit H0; eauto. intros [dst' [sl1' [sl2' [a' [tmp' [P [Q [R S]]]]]]]].
-  TR. subst sl1. rewrite app_ass. eauto.
-  red; auto.
-  intros. rewrite <- app_ass. econstructor. apply S; auto.
-  eapply tr_expr_invariant; eauto. UNCHANGED.
-  eauto. auto. auto. auto. auto. auto. auto. auto. auto. auto. auto.
-  eapply typeof_context; eauto.
-- (* assignop right *)
-  inv H2.
-+ (* for effects *)
-  assert (sl1 = nil) by (eapply tr_simple_expr_nil; eauto). subst sl1; simpl.
-  exploit H1; eauto. intros [dst' [sl1' [sl2' [a' [tmp' [P [Q [R S]]]]]]]].
-  TR. subst sl2. rewrite app_ass. eauto.
-  red; auto.
-  intros. rewrite <- app_ass. change (sl0 ++ sl2') with (nil ++ sl0 ++ sl2'). rewrite app_ass. econstructor.
-  eapply tr_expr_invariant; eauto. UNCHANGED.
-  apply S; auto. auto. eauto. auto. auto. auto. auto. auto. auto.
-+ (* for val *)
-  assert (sl1 = nil) by (eapply tr_simple_expr_nil; eauto). subst sl1; simpl.
-  exploit H1; eauto. intros [dst' [sl1' [sl2' [a' [tmp' [P [Q [R S]]]]]]]].
-  TR. subst sl2. rewrite app_ass. eauto.
-  red; auto.
-  intros. rewrite <- app_ass. change (sl0 ++ sl2') with (nil ++ sl0 ++ sl2'). rewrite app_ass. econstructor.
-  eapply tr_expr_invariant; eauto. UNCHANGED.
-  apply S; auto. eauto. auto. auto. auto. auto. auto. auto. auto. auto. auto. auto. auto.
-- (* postincr *)
-  inv H1.
-+ (* for effects *)
-  exploit H0; eauto. intros [dst' [sl1' [sl2' [a' [tmp' [P [Q [R S]]]]]]]].
-  TR. rewrite Q; rewrite app_ass; eauto. red; auto.
-  intros. rewrite <- app_ass. econstructor; eauto.
-  symmetry; eapply typeof_context; eauto.
-+ (* for val *)
-  exploit H0; eauto. intros [dst' [sl1' [sl2' [a' [tmp' [P [Q [R S]]]]]]]].
-  TR. rewrite Q; rewrite app_ass; eauto. red; auto.
-  intros. rewrite <- app_ass. econstructor; eauto.
-  eapply typeof_context; eauto.
-- (* call left *)
-  inv H1.
-+ (* for effects *)
-  exploit H0; eauto. intros [dst' [sl1' [sl2' [a' [tmp' [P [Q [R S]]]]]]]].
-  TR. rewrite Q; rewrite app_ass; eauto. red; auto.
-  intros. rewrite <- app_ass. econstructor. apply S; auto.
-  eapply tr_exprlist_invariant; eauto. UNCHANGED.
-  auto. auto. auto.
-+ (* for val *)
-  exploit H0; eauto. intros [dst' [sl1' [sl2' [a' [tmp' [P [Q [R S]]]]]]]].
-  TR. rewrite Q; rewrite app_ass; eauto. red; auto.
-  intros. rewrite <- app_ass. econstructor. auto. apply S; auto.
-  eapply tr_exprlist_invariant; eauto. UNCHANGED.
-  auto. auto. auto. auto.
-- (* call right *)
-  inv H2.
-+ (* for effects *)
-  assert (sl1 = nil) by (eapply tr_simple_expr_nil; eauto). subst sl1; simpl.
-  exploit H1; eauto. intros [dst' [sl1' [sl2' [a' [tmp' [P [Q [R S]]]]]]]].
-  TR. rewrite Q; rewrite app_ass; eauto.
-  (*destruct dst'; constructor||contradiction.*)
-  red; auto.
-  intros. rewrite <- app_ass. change (sl3++sl2') with (nil ++ sl3 ++ sl2'). rewrite app_ass. econstructor.
-  eapply tr_expr_invariant; eauto. UNCHANGED.
-  apply S; auto. auto. auto. auto.
-+ (* for val *)
-  assert (sl1 = nil) by (eapply tr_simple_expr_nil; eauto). subst sl1; simpl.
-  exploit H1; eauto. intros [dst' [sl1' [sl2' [a' [tmp' [P [Q [R S]]]]]]]].
-  TR. rewrite Q; rewrite app_ass; eauto.
-  (*destruct dst'; constructor||contradiction.*)
-  red; auto.
-  intros. rewrite <- app_ass. change (sl3++sl2') with (nil ++ sl3 ++ sl2'). rewrite app_ass. econstructor.
-  auto. eapply tr_expr_invariant; eauto. UNCHANGED.
-  apply S; auto.
-  auto. auto. auto. auto.
-- (* builtin *)
-  inv H1.
-+ (* for effects *)
-  exploit H0; eauto. intros [dst' [sl1' [sl2' [a' [tmp' [P [Q [R S]]]]]]]].
-  TR. rewrite Q; rewrite app_ass; eauto.
-  red; auto.
-  intros. rewrite <- app_ass. change (sl3++sl2') with (nil ++ sl3 ++ sl2'). rewrite app_ass. econstructor.
-  apply S; auto. auto.
-+ (* for val *)
-  exploit H0; eauto. intros [dst' [sl1' [sl2' [a' [tmp' [P [Q [R S]]]]]]]].
-  TR. rewrite Q; rewrite app_ass; eauto.
-  red; auto.
-  intros. rewrite <- app_ass. change (sl3++sl2') with (nil ++ sl3 ++ sl2'). rewrite app_ass. econstructor.
-  auto. apply S; auto. auto. auto.
-- (* comma *)
-  inv H1.
-  exploit H0; eauto. intros [dst' [sl1' [sl2' [a' [tmp' [P [Q [R S]]]]]]]].
-  TR. rewrite Q; rewrite app_ass; eauto. red; auto.
-  intros. rewrite <- app_ass. econstructor. apply S; auto.
-  eapply tr_expr_invariant; eauto. UNCHANGED.
-  auto. auto. auto.
-- (* paren *)
-  inv H1.
-+ (* for val *)
-  exploit H0; eauto. intros [dst' [sl1' [sl2' [a' [tmp' [P [Q [R S]]]]]]]].
-  TR. rewrite Q. eauto. red; auto.
-  intros. econstructor; eauto.
-+ (* for effects *)
-  exploit H0; eauto. intros [dst' [sl1' [sl2' [a' [tmp' [P [Q [R S]]]]]]]].
-  TR. rewrite Q. eauto. auto.
-  intros. econstructor; eauto.
-+ (* for set *)
-  exploit H0; eauto. intros [dst' [sl1' [sl2' [a' [tmp' [P [Q [R S]]]]]]]].
-  TR. rewrite Q. eauto. auto.
-  intros. econstructor; eauto.
-- (* cons left *)
-  inv H1.
-  exploit H0; eauto. intros [dst' [sl1' [sl2' [a' [tmp' [P [Q [R S]]]]]]]].
-  TR. subst sl1. rewrite app_ass. eauto.
-  red; auto.
-  intros. rewrite <- app_ass. econstructor. apply S; auto.
-  eapply tr_exprlist_invariant; eauto.  UNCHANGED.
-  auto. auto. auto.
-- (* cons right *)
-  inv H2.
-  assert (sl1 = nil) by (eapply tr_simple_expr_nil; eauto). subst sl1; simpl.
-  exploit H1; eauto. intros [dst' [sl1' [sl2' [a' [tmp' [P [Q [R S]]]]]]]].
-  TR. subst sl2. eauto.
-  red; auto.
-  intros. change sl3 with (nil ++ sl3). rewrite app_ass. econstructor.
-  eapply tr_expr_invariant; eauto. UNCHANGED.
-  apply S; auto.
-  auto. auto. auto.
+    apply leftcontext_leftcontextlist_ind; intros; simpl; iIntros; norm_all.
+    (*base*)
+    - repeat iExists _. iSplitL; eauto. iSplit. iPureIntro; apply app_nil_end.
+      iIntros "* % *". iApply locally_simpl. rewrite <- app_nil_end. eauto.
+    (* deref *)
+    - init H0 e' "HF". iApply locally_simpl. finish_him.
+    (* field *)
+    - init H0 e' "HF". iApply locally_simpl. finish_him.
+    (* rvalof *)
+    - init H0 e' "HF". rewrite (typeof_context _ _ _ H _ _ a0). iApply locally_simpl. finish_him.
+    (* addrof *)
+    - init H0 e' "HF". iApply locally_simpl. finish_him.
+    - init H0 e' "HF". iApply locally_simpl. finish_him.
+    (* binop left *)
+    - iDestruct (proj1 tr_expr_invariant with "HH") as "HC".
+      init H0 e' "HF". iApply (locally_consequence with "HC"). finish_him.
+    (* binop right *)
+    - iAssert (⌜x = nil⌝) as "%". iApply (tr_simple_expr_nil with "HF"); eauto.
+      iDestruct (proj1 tr_expr_invariant with "HF") as "HC".
+      init H1 e' "HH". iApply (locally_consequence with "HC"). finish_him.
+    (* cast *)
+    - init H0 e' "HF". iApply locally_simpl. finish_him.
+    (* seqand *)
+    - destruct dst; norm_all; iDestruct (proj1 tr_expr_invariant with "HF") as "HB"; init H0 e' "HD";
+        iApply (locally_consequence with "HB"); finish_him.
+    (* seqor *)
+    - destruct dst; norm_all; iDestruct (proj1 tr_expr_invariant with "HF") as "HF"; init H0 e' "HD";
+        iApply (locally_consequence with "HF"); finish_him.
+    (* condition *)
+    - destruct dst; norm_all.
+      + iDestruct (locally_and with "[HF]") as "HB". iSplit.
+        iDestruct "HF" as "[HB _]". iApply (proj1 tr_expr_invariant with "HB").
+        iDestruct "HF" as "[_ HB]". iApply (proj1 tr_expr_invariant with "HB").
+        init H0 e' "HD". iApply (locally_consequence with "HB"). finish_him.
+      + iDestruct (proj1 tr_expr_invariant with "HF") as "HF".
+        iDestruct (proj1 tr_expr_invariant with "HH") as "HH".
+        init H0 e' "HD".  iApply (locally_delete_2 with "HH HF"). finish_him.
+      + iDestruct (locally_and with "[HH]") as "HH". iSplit.
+        iDestruct "HH" as "[HB _]". iApply (proj1 tr_expr_invariant with "HB").
+        iDestruct "HH" as "[_ HB]". iApply (proj1 tr_expr_invariant with "HB").
+        init H0 e' "HF". iApply (locally_consequence with "HH"). finish_him.
+    - destruct dst; norm_all.
+      + iDestruct (proj1 tr_expr_invariant with "HF") as "HF".
+        init H0 e' "HD". iApply (locally_consequence with "HF").
+        rewrite (typeof_context _ _ _ H _ _ a). finish_him.
+      + iDestruct (proj1 tr_expr_invariant with "HF") as "HF". init H0 e' "HD".
+        iApply (locally_consequence with "HF"). finish_him.
+      + iDestruct (proj1 tr_expr_invariant with "HF") as "HF". init H0 e' "HD".
+        iApply (locally_consequence with "HF"). rewrite (typeof_context _ _ _ H _ _ a). finish_him.
+    - destruct dst; norm_all; iDestruct (tr_simple_expr_nil with "HD [] []") as "%"; auto;
+        iDestruct (proj1 tr_expr_invariant with "HD") as "HD"; init H1 e' "HF";
+         iApply (locally_consequence with "HD"); finish_him.
+    - destruct dst; norm_all.
+      + iDestruct (proj1 tr_expr_invariant with "HH") as "HH". init H0 e' "HF".
+        rewrite (typeof_context _ _ _ H e' e _). iApply (locally_consequence with "HH"); finish_him.
+        auto.
+      + iDestruct (proj1 tr_expr_invariant with "HF") as "HF". init H0 e' "HD".
+        rewrite (typeof_context _ _ _ H e' e _). iApply (locally_consequence with "HF"); finish_him.
+        auto.
+      + iDestruct (proj1 tr_expr_invariant with "HH") as "HH". init H0 e' "HF".
+        rewrite (typeof_context _ _ _ H e' e _). iApply (locally_consequence with "HH"); finish_him.
+        auto.
+    - destruct dst; norm_all.
+      + iDestruct (tr_simple_expr_nil with "HF [] []") as "%"; auto.
+        iDestruct (proj1 tr_expr_invariant with "HF") as "HF". init H1 e' "HH".
+        iApply (locally_consequence with "HF"); finish_him.
+      + iDestruct (tr_simple_expr_nil with "HD [] []") as "%"; auto.
+        iDestruct (proj1 tr_expr_invariant with "HD") as "HD". init H1 e' "HF".
+        iApply (locally_consequence with "HD"); finish_him.
+      + iDestruct (tr_simple_expr_nil with "HF [] []") as "%"; auto.
+        iDestruct (proj1 tr_expr_invariant with "HF") as "HF". init H1 e' "HH".
+        iApply (locally_consequence with "HF"); finish_him.
+    - destruct dst; norm_all; init H0 e' "HD"; iApply locally_simpl;
+        rewrite (typeof_context _ _ _ H e e' _); auto; iIntros "* HA !>"; repeat iExists _; iFrame;
+          repeat iExists _; iSplitL; auto; rewrite app_ass; auto.
+    - destruct dst; norm_all.
+      + iDestruct (proj2 tr_expr_invariant with "HJ") as "HJ". init H0 e' "HH".
+        iApply (locally_consequence with "HJ"). finish_him.
+      + iDestruct (proj2 tr_expr_invariant with "HF") as "HF". init H0 e' "HD".
+        iApply (locally_consequence with "HF"). finish_him.
+      + iDestruct (proj2 tr_expr_invariant with "HJ") as "HJ". init H0 e' "HH".
+        iApply (locally_consequence with "HJ"). finish_him.
+    - destruct dst; norm_all.
+      + iDestruct (tr_simple_expr_nil with "HH [] []") as "%"; auto.
+        iDestruct (proj1 tr_expr_invariant with "HH") as "HH". init H1 e' "HJ".
+        iApply (locally_consequence with "HH"). finish_him.
+      + iDestruct (tr_simple_expr_nil with "HD [] []") as "%"; auto.
+        iDestruct (proj1 tr_expr_invariant with "HD") as "HD". init H1 e' "HF".
+        iApply (locally_consequence with "HD"). finish_him.
+      + iDestruct (tr_simple_expr_nil with "HH [] []") as "%"; auto.
+        iDestruct (proj1 tr_expr_invariant with "HH") as "HH". init H1 e' "HJ".
+        iApply (locally_consequence with "HH"). finish_him.
+    - destruct dst; norm_all.
+      + init H0 e' "HF"; iApply locally_simpl; finish_him.
+      + init H0 e' "HD"; iApply locally_simpl; finish_him.
+      + init H0 e' "HF"; iApply locally_simpl; finish_him.
+    - iDestruct (proj1 tr_expr_invariant with "HF") as "HF". init H0 e' "HD".
+      iApply (locally_consequence with "HF"). finish_him.
+    - destruct dst; norm_all.
+      + init H0 e' "HD". iApply locally_simpl. finish_him.
+      + init H0 e' "HB". iApply locally_simpl. finish_him.
+      + destruct (Pos.eq_dec x0 (sd_temp sd)) eqn:?; norm_all.
+        * init H0 e' "HB". iApply locally_simpl. finish_him.
+          instantiate (2 := (sd_temp sd)). rewrite Heqs. iFrame.
+        * init H0 e' "HD". iApply locally_simpl. finish_him.
+          instantiate (2 := x0). rewrite Heqs. iFrame.
+    - iDestruct (proj2 tr_expr_invariant with "HD") as "HD". init H0 e' "HB".
+      iApply (locally_consequence with "HD"). finish_him.
+    - iDestruct (tr_simple_expr_nil with "HB [] []") as "%"; auto.
+      iDestruct (proj1 tr_expr_invariant with "HB") as "HB". init H1 e' "HD".
+      iApply (locally_consequence with "HB"). finish_him.
 Qed.
 
 Theorem tr_expr_leftcontext:
-  forall C le r dst sl a tmps,
-  leftcontext RV RV C ->
-  tr_expr le dst (C r) sl a tmps ->
-  exists dst', exists sl1, exists sl2, exists a', exists tmp',
-  tr_expr le dst' r sl1 a' tmp'
-  /\ sl = sl1 ++ sl2
-  /\ incl tmp' tmps
-  /\ (forall le' r' sl3,
-        tr_expr le' dst' r' sl3 a' tmp' ->
-        (forall id, ~In id tmp' -> le'!id = le!id) ->
-        Csyntax.typeof r' = Csyntax.typeof r ->
-        tr_expr le' dst (C r') (sl3 ++ sl2) a tmps).
+  forall from to C, leftcontext from to C ->
+  forall le e dst sl a,
+  ⊢ tr_expr le dst (C e) sl a -∗
+  ∃ dst' sl1 sl2 a',
+    tr_expr le dst' e sl1 a'
+    ∗ ⌜ sl = sl1 ++ sl2 ⌝
+    ∗ ∀ e',
+        \⌜ Csyntax.typeof e' = Csyntax.typeof e ⌝ -∗
+        (∀ sl3,
+        locally le (fun le' => tr_expr le' dst' e' sl3 a'
+                              -∗ tr_expr le' dst (C e') (sl3 ++ sl2) a)).
 Proof.
-  intros. eapply (proj1 tr_expr_leftcontext_rec); eauto.
-Qed.
-
-Theorem tr_top_leftcontext:
-  forall e le m dst rtop sl a tmps,
-  tr_top tge e le m dst rtop sl a tmps ->
-  forall r C,
-  rtop = C r ->
-  leftcontext RV RV C ->
-  exists dst', exists sl1, exists sl2, exists a', exists tmp',
-  tr_top tge e le m dst' r sl1 a' tmp'
-  /\ sl = sl1 ++ sl2
-  /\ incl tmp' tmps
-  /\ (forall le' m' r' sl3,
-        tr_expr le' dst' r' sl3 a' tmp' ->
-        (forall id, ~In id tmp' -> le'!id = le!id) ->
-        Csyntax.typeof r' = Csyntax.typeof r ->
-        tr_top tge e le' m' dst (C r') (sl3 ++ sl2) a tmps).
-Proof.
-  induction 1; intros.
-(* val for val *)
-  inv H2; inv H1.
-  exists For_val; econstructor; econstructor; econstructor; econstructor.
-  split. apply tr_top_val_val; eauto.
-  split. instantiate (1 := nil); auto.
-  split. apply incl_refl.
-  intros. rewrite <- app_nil_end. constructor; auto.
-(* base *)
-  subst r. exploit tr_expr_leftcontext; eauto.
-  intros [dst' [sl1 [sl2 [a' [tmp' [P [Q [R S]]]]]]]].
-  exists dst'; exists sl1; exists sl2; exists a'; exists tmp'.
-  split. apply tr_top_base; auto.
-  split. auto. split. auto.
-  intros. apply tr_top_base. apply S; auto.
+  exact (proj1 tr_expr_leftcontext_rec).
 Qed.
 
 (** Semantics of smart constructors *)
@@ -786,8 +664,11 @@ Proof.
   destruct (Mem.weak_valid_pointer m1 b (Ptrofs.unsigned i)); inv H.
   destruct (Mem.weak_valid_pointer m2 b (Ptrofs.unsigned i)); inv H0.
   auto.
-- destruct v; try congruence. 
+- destruct v; try congruence.
   destruct (negb Archi.ptr64); try discriminate.
+  destruct (Mem.weak_valid_pointer m1 b (Ptrofs.unsigned i)); inv H.
+  destruct (Mem.weak_valid_pointer m2 b (Ptrofs.unsigned i)); inv H0.
+  auto.
   destruct (Mem.weak_valid_pointer m1 b (Ptrofs.unsigned i)); inv H.
   destruct (Mem.weak_valid_pointer m2 b (Ptrofs.unsigned i)); inv H0.
   auto.
@@ -809,9 +690,9 @@ Lemma static_bool_val_sound:
 Proof.
   assert (A: forall b ofs, Mem.weak_valid_pointer Mem.empty b ofs = false).
   { unfold Mem.weak_valid_pointer, Mem.valid_pointer, proj_sumbool; intros.
-    rewrite ! pred_dec_false by (apply Mem.perm_empty). auto. }  
+    rewrite ! pred_dec_false; auto; apply Mem.perm_empty. }
   intros until b; unfold bool_val.
-  destruct (classify_bool t); destruct v; destruct Archi.ptr64 eqn:SF; auto.
+  destruct (classify_bool t0); destruct v; destruct Archi.ptr64 eqn:SF; auto.
 - rewrite A; congruence.
 - simpl; rewrite A; congruence.
 Qed.
@@ -840,17 +721,17 @@ Lemma step_make_set:
   eval_lvalue tge e le m a b ofs ->
   typeof a = ty ->
   step1 tge (State f (make_set id a) k e le m)
-          t (State f Sskip k e (PTree.set id v le) m).
+          t (State f Sskip k e (Maps.PTree.set id v le) m).
 Proof.
   intros. exploit deref_loc_translated; eauto. rewrite <- H1.
   unfold make_set. destruct (chunk_for_volatile_type (typeof a)) as [chunk|].
 (* volatile case *)
-  intros. change (PTree.set id v le) with (set_opttemp (Some id) v le). econstructor.
+  intros. change (Maps.PTree.set id v le) with (set_opttemp (Some id) v le). econstructor.
   econstructor. constructor. eauto.
   simpl. unfold sem_cast. simpl. eauto. constructor.
   simpl. econstructor; eauto.
 (* nonvolatile case *)
-  intros [A B]. subst t. constructor. eapply eval_Elvalue; eauto.
+  intros [A B]. subst t0. constructor. eapply eval_Elvalue; eauto.
 Qed.
 
 Lemma step_make_assign:
@@ -872,7 +753,7 @@ Proof.
   econstructor; eauto. rewrite H3; eauto. constructor.
   simpl. econstructor; eauto.
 (* nonvolatile case *)
-  intros [A B]. subst t. econstructor; eauto. congruence.
+  intros [A B]. subst t0. econstructor; eauto. congruence.
 Qed.
 
 Fixpoint Kseqlist (sl: list statement) (k: cont) :=
@@ -900,32 +781,29 @@ Proof.
 Qed.
 
 Lemma step_tr_rvalof:
-  forall ty m b ofs t v e le a sl a' tmp f k,
+  forall ty m b ofs t v e le a sl a' f k,
   Csem.deref_loc ge ty m b ofs t v ->
   eval_lvalue tge e le m a b ofs ->
-  tr_rvalof ty a sl a' tmp ->
   typeof a = ty ->
-  exists le',
-    star step1 tge (State f Sskip (Kseqlist sl k) e le m)
+  ⊢ tr_rvalof ty a sl a' -∗
+  ∃ le',
+    ⌜star step1 tge (State f Sskip (Kseqlist sl k) e le m)
                  t (State f Sskip k e le' m)
   /\ eval_expr tge e le' m a' v
-  /\ typeof a' = typeof a
-  /\ forall x, ~In x tmp -> le'!x = le!x.
+  /\ typeof a' = typeof a ⌝.
 Proof.
-  intros. inv H1.
-  (* not volatile *)
-  exploit deref_loc_translated; eauto. unfold chunk_for_volatile_type; rewrite H3.
-  intros [A B]. subst t.
-  exists le; split. apply star_refl.
-  split. eapply eval_Elvalue; eauto.
-  auto.
-  (* volatile *)
-  intros. exists (PTree.set t0 v le); split.
-  simpl. eapply star_two. econstructor. eapply step_make_set; eauto. traceEq.
-  split. constructor. apply PTree.gss.
-  split. auto.
-  intros. apply PTree.gso. congruence.
+  iIntros "* % % % HA". unfold tr_rvalof.
+  destruct (type_is_volatile ty) eqn:?; norm_all.
+  - subst. iExists (Maps.PTree.set _ v le). iSplitR.
+    + iPureIntro. simpl. eapply star_two. econstructor. eapply step_make_set; eauto. traceEq.
+    + iPureIntro. split. constructor. apply Maps.PTree.gss. reflexivity.
+  - subst. exploit deref_loc_translated; eauto. intro.
+    unfold chunk_for_volatile_type in H1. rewrite Heqb0 in H1. destruct H1. subst.
+    iExists le. iSplit; eauto.
+    iPureIntro. apply star_refl. iPureIntro. split. eapply eval_Elvalue; eauto.
+    reflexivity.
 Qed.
+
 
 (** Matching between continuations *)
 
@@ -972,15 +850,15 @@ Inductive match_cont : Csem.cont -> cont -> Prop :=
       match_cont_exp dest a k tk ->
       match_cont (Csem.Kcall f e C ty k)
                  (Kcall optid tf e le (Kseqlist sl tk))
-(*
-  | match_Kcall_some: forall f e C ty k dst tf le sl tk a dest tmps,
-      transl_function f = Errors.OK tf ->
-      leftcontext RV RV C ->
-      (forall v m, tr_top tge e (PTree.set dst v le) m dest (C (C.Eval v ty)) sl a tmps) ->
-      match_cont_exp dest a k tk ->
-      match_cont (Csem.Kcall f e C ty k)
-                 (Kcall (Some dst) tf e le (Kseqlist sl tk))
-*)
+(* *)
+(*   | match_Kcall_some: forall f e C ty k dst tf le sl tk a dest tmps, *)
+(*       transl_function f = Errors.OK tf -> *)
+(*       leftcontext RV RV C -> *)
+(*       (forall v m, tr_top tge e (PTree.set dst v le) m dest (C (C.Eval v ty)) sl a tmps) -> *)
+(*       match_cont_exp dest a k tk -> *)
+(*       match_cont (Csem.Kcall f e C ty k) *)
+(*                  (Kcall (Some dst) tf e le (Kseqlist sl tk)) *)
+(* *)
 
 with match_cont_exp : destination -> expr -> Csem.cont -> cont -> Prop :=
   | match_Kdo: forall k a tk,
@@ -990,7 +868,8 @@ with match_cont_exp : destination -> expr -> Csem.cont -> cont -> Prop :=
       match_cont k tk ->
       match_cont_exp For_val a (Csem.Kifthenelse Csyntax.Sskip Csyntax.Sskip k) (Kseq Sskip tk)
   | match_Kifthenelse_1: forall a s1 s2 k ts1 ts2 tk,
-      tr_stmt s1 ts1 -> tr_stmt s2 ts2 ->
+      tr_stmt s1 ts1 ->
+      tr_stmt s2 ts2 ->
       match_cont k tk ->
       match_cont_exp For_val a (Csem.Kifthenelse s1 s2 k) (Kseq (Sifthenelse a ts1 ts2) tk)
   | match_Kwhile1: forall r s k s' a ts tk,
@@ -1030,12 +909,13 @@ Lemma match_cont_call:
   match_cont k tk ->
   match_cont (Csem.call_cont k) (call_cont tk).
 Proof.
-  induction 1; simpl; auto. constructor. econstructor; eauto.
+  induction 1; simpl; auto. constructor. econstructor; auto.
 Qed.
+
 
 (** Matching between states *)
 
-Inductive match_states: Csem.state -> state -> Prop :=
+Inductive match_states: Csem.state -> Clight.state -> Prop :=
   | match_exprstates: forall f r k e m tf sl tk le dest a tmps,
       tr_function f tf ->
       tr_top tge e le m dest r sl a tmps ->
@@ -1067,7 +947,7 @@ Lemma tr_select_switch:
   tr_lblstmts ls tls ->
   tr_lblstmts (Csem.select_switch n ls) (select_switch n tls).
 Proof.
-  assert (DFL: forall ls tls,
+ assert (DFL: forall ls tls,
       tr_lblstmts ls tls ->
       tr_lblstmts (Csem.select_switch_default ls) (select_switch_default tls)).
   { induction 1; simpl. constructor. destruct c; auto. constructor; auto. }
@@ -1089,6 +969,7 @@ Proof.
   destruct CASE as [tls' [P Q]]. rewrite P. auto.
   rewrite CASE. apply DFL; auto.
 Qed.
+
 
 Lemma tr_seq_of_labeled_statement:
   forall ls tls,
@@ -1151,9 +1032,11 @@ Proof.
 Qed.
 
 Lemma tr_rvalof_nolabel:
-  forall ty a sl a' tmp, tr_rvalof ty a sl a' tmp -> nolabel_list sl.
+  forall ty a sl a', ⊢ tr_rvalof ty a sl a' -∗ ⌜ nolabel_list sl ⌝.
 Proof.
-  destruct 1; simpl; intuition. apply make_set_nolabel.
+  iIntros. unfold tr_rvalof.
+  destruct (type_is_volatile ty) eqn:?; norm_all; subst; iPureIntro; repeat constructor.
+  apply make_set_nolabel.
 Qed.
 
 Lemma nolabel_do_set:
@@ -1171,7 +1054,7 @@ Qed.
 Ltac NoLabelTac :=
   match goal with
   | [ |- nolabel_list nil ] => exact I
-  | [ |- nolabel_list (final _ _) ] => apply nolabel_final (*; NoLabelTac*)
+  | [ |- nolabel_list (final _ _) ] => apply nolabel_final
   | [ |- nolabel_list (_ :: _) ] => simpl; split; NoLabelTac
   | [ |- nolabel_list (_ ++ _) ] => apply nolabel_list_app; NoLabelTac
   | [ H: _ -> nolabel_list ?x |- nolabel_list ?x ] => apply H; NoLabelTac
@@ -1179,31 +1062,61 @@ Ltac NoLabelTac :=
   | [ |- nolabel (makeif _ _ _) ] => apply makeif_nolabel; NoLabelTac
   | [ |- nolabel (make_set _ _) ] => apply make_set_nolabel
   | [ |- nolabel (make_assign _ _) ] => apply make_assign_nolabel
-  | [ |- nolabel _ ] => red; intros; simpl; auto
+  | [ |- nolabel_list (do_set _ _) ] => apply nolabel_do_set
+  | [ |- nolabel _ ] => intro; simpl; auto
   | [ |- _ /\ _ ] => split; NoLabelTac
   | _ => auto
   end.
 
+Ltac apply_ind_label l h :=
+  match type of l with
+  | Csyntax.expr =>
+    match goal with
+    | H : forall _ _ _ _, bi_emp_valid (tr_expr _ _ l _ _ -∗ _) |- _ => iDestruct (H with h) as "%"
+    end
+  | exprlist =>
+    match goal with
+    | H : forall _ _ _, bi_emp_valid (tr_exprlist _ l _ _ -∗ _) |- _ => iDestruct (H with h) as "%"
+    end
+  | expr => iDestruct (tr_rvalof_nolabel with h) as "%"
+  end.
+
+
 Lemma tr_find_label_expr:
-  (forall le dst r sl a tmps, tr_expr le dst r sl a tmps -> nolabel_list sl)
-/\(forall le rl sl al tmps, tr_exprlist le rl sl al tmps -> nolabel_list sl).
+  (forall r le dst sl a, ⊢ tr_expr le dst r sl a -∗ ⌜ nolabel_list sl ⌝)
+/\(forall rl le sl al, ⊢ tr_exprlist le rl sl al -∗ ⌜ nolabel_list sl ⌝).
 Proof.
-  apply tr_expr_exprlist; intros; NoLabelTac.
-  apply nolabel_do_set.
-  eapply tr_rvalof_nolabel; eauto.
-  apply nolabel_do_set.
-  apply nolabel_do_set.
-  eapply tr_rvalof_nolabel; eauto.
-  eapply tr_rvalof_nolabel; eauto.
-  eapply tr_rvalof_nolabel; eauto.
+  apply tr_expr_exprlist; intros; simpl; iIntros; norm_all; apply_ind apply_ind_label; subst;
+    try(iPureIntro; NoLabelTac; fail).
+  - destruct dst; norm_all; subst; NoLabelTac. iDestruct "HB" as "[_ HA]". norm_all.
+    subst; iPureIntro; NoLabelTac.
+  - destruct dst; norm_all; apply_ind apply_ind_label; subst; iPureIntro; NoLabelTac.
+  - destruct dst; norm_all; apply_ind apply_ind_label; subst; iPureIntro; NoLabelTac.
+  - destruct dst; norm_all; apply_ind apply_ind_label; subst.
+    + iDestruct (H0 with "[HF]") as "%". iDestruct "HF" as "[HD _]"; auto.
+      iDestruct (H1 with "[HF]") as "%". iDestruct "HF" as "[_ HD]"; auto.
+      subst. iPureIntro. NoLabelTac.
+    + subst. iPureIntro. NoLabelTac.
+    + iDestruct (H0 with "[HH]") as "%". iDestruct "HH" as "[HC _]"; auto.
+      iDestruct (H1 with "[HH]") as "%". iDestruct "HH" as "[_ HC]"; auto.
+      subst. iPureIntro. NoLabelTac.
+  - destruct dst; norm_all; apply_ind apply_ind_label; subst; iPureIntro; NoLabelTac.
+  - destruct dst; norm_all; apply_ind apply_ind_label; subst; iPureIntro; NoLabelTac.
+  - destruct dst; norm_all; apply_ind apply_ind_label; subst; iPureIntro; NoLabelTac.
+  - destruct dst; norm_all; apply_ind apply_ind_label; subst; iPureIntro; NoLabelTac.
+  - destruct dst; norm_all; apply_ind apply_ind_label; subst; iPureIntro; NoLabelTac.
+  - destruct dst; norm_all; apply_ind apply_ind_label; auto.
+    destruct (Pos.eq_dec x0 (sd_temp sd)); norm_all; apply_ind apply_ind_label; auto.
+  - destruct a. subst. NoLabelTac.
 Qed.
 
 Lemma tr_find_label_top:
-  forall e le m dst r sl a tmps,
-  tr_top tge e le m dst r sl a tmps -> nolabel_list sl.
+  forall e le m dst r sl a tmp,
+    tr_top tge e le m dst r sl a tmp -> nolabel_list sl.
 Proof.
-  induction 1; intros; NoLabelTac.
-  eapply (proj1 tr_find_label_expr); eauto.
+  intros. inv H; NoLabelTac.
+  apply (soundness1 tmp). iIntros "HA". apply soundness3 in H0.
+  iDestruct (H0 with "HA") as "HA". iDestruct (proj1 tr_find_label_expr with "HA") as "$"; auto.
 Qed.
 
 Lemma tr_find_label_expression:
@@ -1211,8 +1124,8 @@ Lemma tr_find_label_expression:
 Proof.
   intros. inv H.
   assert (nolabel (makeseq sl)). apply makeseq_nolabel.
-  eapply tr_find_label_top with (e := empty_env) (le := PTree.empty val) (m := Mem.empty).
-  eauto. apply H.
+  eapply (tr_find_label_top empty_env (Maps.PTree.empty val) Mem.empty); eauto.
+  apply H.
 Qed.
 
 Lemma tr_find_label_expr_stmt:
@@ -1220,23 +1133,19 @@ Lemma tr_find_label_expr_stmt:
 Proof.
   intros. inv H.
   assert (nolabel (makeseq sl)). apply makeseq_nolabel.
-  eapply tr_find_label_top with (e := empty_env) (le := PTree.empty val) (m := Mem.empty).
-  eauto. apply H.
+  eapply (tr_find_label_top empty_env (Maps.PTree.empty val) Mem.empty); eauto.
+  apply H.
 Qed.
 
 Lemma tr_find_label_if:
-  forall r s,
-  tr_if r Sskip Sbreak s ->
-  forall k, find_label lbl s k = None.
+  forall r s, tr_if r Sskip Sbreak s -> forall k, find_label lbl s k = None.
 Proof.
   intros. inv H.
   assert (nolabel (makeseq (sl ++ makeif a Sskip Sbreak :: nil))).
   apply makeseq_nolabel.
   apply nolabel_list_app.
-  eapply tr_find_label_top with (e := empty_env) (le := PTree.empty val) (m := Mem.empty).
-  eauto.
-  simpl; split; auto. apply makeif_nolabel. red; simpl; auto. red; simpl; auto.
-  apply H.
+  eapply (tr_find_label_top empty_env (Maps.PTree.empty val) Mem.empty); eauto.
+  NoLabelTac. apply H.
 Qed.
 
 Lemma tr_find_label:
@@ -1422,557 +1331,822 @@ Qed.
 
 (** Forward simulation for expressions. *)
 
-Lemma tr_val_gen:
-  forall le dst v ty a tmp,
-  typeof a = ty ->
-  (forall tge e le' m,
-      (forall id, In id tmp -> le'!id = le!id) ->
-      eval_expr tge e le' m a v) ->
-  tr_expr le dst (Csyntax.Eval v ty) (final dst a) a tmp.
+Ltac apply_ind_dest l h :=
+    match goal with
+    | H : forall _ _ _ _, bi_emp_valid (tr_expr _ _ l _ _ -∗ _) |- _ =>
+      iDestruct (H with h) as h
+    | _ => fail "No rec"
+    end.
+
+
+Lemma tr_expr_dest : forall r le dst sl a, ⊢ tr_expr le dst r sl a -∗ <absorb> dest_below dst.
 Proof.
-  intros. destruct dst; simpl; econstructor; auto.
+  induction r; iIntros; simpl; destruct dst; norm_all; apply_ind apply_ind_dest; simpl; auto.
+  - iDestruct "HB" as "[$ _]".
+  - contradiction.
+  - destruct (Pos.eq_dec x0 (sd_temp sd)); norm_all; subst; apply_ind apply_ind_dest; simpl; auto.
 Qed.
+
+Lemma pure_next_step P (R : Prop) (Q : iProp) :
+  (forall tmp, Q () tmp -> R) -> (⊢P -∗ Q) -> (P -∗ ⌜R⌝)%stdpp.
+Proof.
+  intros. apply instance_heap. intros. apply (H tmps). apply soundness2.
+  apply soundness3 in H1. iIntros "HA". iDestruct (H1 with "HA") as "HA". iApply (H0 with "HA").
+Qed.
+
+Ltac iConstructor :=
+  iStopProof; eapply pure_next_step;
+  [ let tmp := fresh in
+    let H := fresh in
+    intros tmp H; econstructor; eauto; econstructor; eapply H| idtac].
 
 Lemma estep_simulation:
   forall S1 t S2, Cstrategy.estep ge S1 t S2 ->
   forall S1' (MS: match_states S1 S1'),
   exists S2',
-     (plus step1 tge S1' t S2' \/
-       (star step1 tge S1' t S2' /\ measure S2 < measure S1)%nat)
+     (Smallstep.plus step1 tge S1' t S2' \/
+       (Smallstep.star step1 tge S1' t S2' /\ measure S2 < measure S1)%nat)
   /\ match_states S2 S2'.
 Proof.
   induction 1; intros; inv MS.
-(* expr *)
-  assert (tr_expr le dest r sl a tmps).
-    inv H9. contradiction. auto.
-  exploit tr_simple_rvalue; eauto. destruct dest.
-  (* for val *)
-  intros [SL1 [TY1 EV1]]. subst sl.
-  econstructor; split.
-  right; split. apply star_refl. destruct r; simpl; (contradiction || lia).
-  econstructor; eauto.
-  instantiate (1 := tmps). apply tr_top_val_val; auto.
-  (* for effects *)
-  intros SL1. subst sl.
-  econstructor; split.
-  right; split. apply star_refl. destruct r; simpl; (contradiction || lia).
-  econstructor; eauto.
-  instantiate (1 := tmps). apply tr_top_base. constructor.
-  (* for set *)
-  inv H10.
-(* rval volatile *)
-  exploit tr_top_leftcontext; eauto. clear H11.
-  intros [dst' [sl1 [sl2 [a' [tmp' [P [Q [R S]]]]]]]].
-  inv P. inv H2. inv H7; try congruence.
-  exploit tr_simple_lvalue; eauto. intros [SL [TY EV]]. subst sl0; simpl.
-  econstructor; split.
-  left. eapply plus_two. constructor. eapply step_make_set; eauto. traceEq.
-  econstructor; eauto.
-  change (final dst' (Etempvar t0 (Csyntax.typeof l)) ++ sl2) with (nil ++ (final dst' (Etempvar t0 (Csyntax.typeof l)) ++ sl2)).
-  apply S. apply tr_val_gen. auto.
-  intros. constructor. rewrite H5; auto. apply PTree.gss.
-  intros. apply PTree.gso. red; intros; subst; elim H5; auto.
-  auto.
-(* seqand true *)
-  exploit tr_top_leftcontext; eauto. clear H9.
-  intros [dst' [sl1 [sl2 [a' [tmp' [P [Q [R S]]]]]]]].
-  inv P. inv H2.
-  (* for val *)
-  exploit tr_simple_rvalue; eauto. intros [SL [TY EV]].
-  subst sl0; simpl Kseqlist.
-  econstructor; split.
-  left. eapply plus_left. constructor.
-  eapply star_trans. apply step_makeif with (b := true) (v1 := v); auto. congruence.
-  apply push_seq. reflexivity. reflexivity.
-  rewrite <- Kseqlist_app.
-  eapply match_exprstates; eauto.
-  apply S. apply tr_paren_val with (a1 := a2); auto.
-  apply tr_expr_monotone with tmp2; eauto. auto. auto.
-  (* for effects *)
-  exploit tr_simple_rvalue; eauto. intros [SL [TY EV]].
-  subst sl0; simpl Kseqlist.
-  econstructor; split.
-  left. eapply plus_left. constructor.
-  eapply star_trans. apply step_makeif with (b := true) (v1 := v); auto. congruence.
-  apply push_seq. reflexivity. reflexivity.
-  rewrite <- Kseqlist_app.
-  eapply match_exprstates; eauto.
-  apply S. apply tr_paren_effects with (a1 := a2); auto.
-  apply tr_expr_monotone with tmp2; eauto. auto. auto.
-  (* for set *)
-  exploit tr_simple_rvalue; eauto. intros [SL [TY EV]].
-  subst sl0; simpl Kseqlist.
-  econstructor; split.
-  left. eapply plus_left. constructor.
-  eapply star_trans. apply step_makeif with (b := true) (v1 := v); auto. congruence.
-  apply push_seq. reflexivity. reflexivity.
-  rewrite <- Kseqlist_app.
-  eapply match_exprstates; eauto.
-  apply S. apply tr_paren_set with (a1 := a2) (t := sd_temp sd); auto.
-  apply tr_expr_monotone with tmp2; eauto. auto. auto.
-(* seqand false *)
-  exploit tr_top_leftcontext; eauto. clear H9.
-  intros [dst' [sl1 [sl2 [a' [tmp' [P [Q [R S]]]]]]]].
-  inv P. inv H2.
-  (* for val *)
-  exploit tr_simple_rvalue; eauto. intros [SL [TY EV]].
-  subst sl0; simpl Kseqlist.
-  econstructor; split.
-  left. eapply plus_left. constructor.
-  eapply star_trans. apply step_makeif with (b := false) (v1 := v); auto. congruence.
-  apply star_one. constructor. constructor. reflexivity. reflexivity.
-  eapply match_exprstates; eauto.
-  change sl2 with (nil ++ sl2). apply S. econstructor; eauto.
-  intros. constructor. rewrite H2. apply PTree.gss. auto.
-  intros. apply PTree.gso. congruence.
-  auto.
-  (* for effects *)
-  exploit tr_simple_rvalue; eauto. intros [SL [TY EV]].
-  subst sl0; simpl Kseqlist.
-  econstructor; split.
-  left. eapply plus_left. constructor.
-  apply step_makeif with (b := false) (v1 := v); auto. congruence.
-  reflexivity.
-  eapply match_exprstates; eauto.
-  change sl2 with (nil ++ sl2). apply S. econstructor; eauto.
-  auto. auto.
-  (* for set *)
-  exploit tr_simple_rvalue; eauto. intros [SL [TY EV]].
-  subst sl0; simpl Kseqlist.
-  econstructor; split.
-  left. eapply plus_left. constructor.
-  eapply star_trans. apply step_makeif with (b := false) (v1 := v); auto. congruence.
-  apply push_seq. reflexivity. reflexivity.
-  rewrite <- Kseqlist_app.
-  eapply match_exprstates; eauto.
-  apply S. econstructor; eauto. intros. constructor. auto. auto.
-(* seqor true *)
-  exploit tr_top_leftcontext; eauto. clear H9.
-  intros [dst' [sl1 [sl2 [a' [tmp' [P [Q [R S]]]]]]]].
-  inv P. inv H2.
-  (* for val *)
-  exploit tr_simple_rvalue; eauto. intros [SL [TY EV]].
-  subst sl0; simpl Kseqlist.
-  econstructor; split.
-  left. eapply plus_left. constructor.
-  eapply star_trans. apply step_makeif with (b := true) (v1 := v); auto. congruence.
-  apply star_one. constructor. constructor. reflexivity. reflexivity.
-  eapply match_exprstates; eauto.
-  change sl2 with (nil ++ sl2). apply S. econstructor; eauto.
-  intros. constructor. rewrite H2. apply PTree.gss. auto.
-  intros. apply PTree.gso. congruence.
-  auto.
-  (* for effects *)
-  exploit tr_simple_rvalue; eauto. intros [SL [TY EV]].
-  subst sl0; simpl Kseqlist.
-  econstructor; split.
-  left. eapply plus_left. constructor.
-  apply step_makeif with (b := true) (v1 := v); auto. congruence.
-  reflexivity.
-  eapply match_exprstates; eauto.
-  change sl2 with (nil ++ sl2). apply S. econstructor; eauto.
-  auto. auto.
-  (* for set *)
-  exploit tr_simple_rvalue; eauto. intros [SL [TY EV]].
-  subst sl0; simpl Kseqlist.
-  econstructor; split.
-  left. eapply plus_left. constructor.
-  eapply star_trans. apply step_makeif with (b := true) (v1 := v); auto. congruence.
-  apply push_seq. reflexivity. reflexivity.
-  rewrite <- Kseqlist_app.
-  eapply match_exprstates; eauto.
-  apply S. econstructor; eauto. intros. constructor. auto. auto.
-(* seqand false *)
-  exploit tr_top_leftcontext; eauto. clear H9.
-  intros [dst' [sl1 [sl2 [a' [tmp' [P [Q [R S]]]]]]]].
-  inv P. inv H2.
-  (* for val *)
-  exploit tr_simple_rvalue; eauto. intros [SL [TY EV]].
-  subst sl0; simpl Kseqlist.
-  econstructor; split.
-  left. eapply plus_left. constructor.
-  eapply star_trans. apply step_makeif with (b := false) (v1 := v); auto. congruence.
-  apply push_seq. reflexivity. reflexivity.
-  rewrite <- Kseqlist_app.
-  eapply match_exprstates; eauto.
-  apply S. apply tr_paren_val with (a1 := a2); auto.
-  apply tr_expr_monotone with tmp2; eauto. auto. auto.
-  (* for effects *)
-  exploit tr_simple_rvalue; eauto. intros [SL [TY EV]].
-  subst sl0; simpl Kseqlist.
-  econstructor; split.
-  left. eapply plus_left. constructor.
-  eapply star_trans. apply step_makeif with (b := false) (v1 := v); auto. congruence.
-  apply push_seq. reflexivity. reflexivity.
-  rewrite <- Kseqlist_app.
-  eapply match_exprstates; eauto.
-  apply S. apply tr_paren_effects with (a1 := a2); auto.
-  apply tr_expr_monotone with tmp2; eauto. auto. auto.
-  (* for set *)
-  exploit tr_simple_rvalue; eauto. intros [SL [TY EV]].
-  subst sl0; simpl Kseqlist.
-  econstructor; split.
-  left. eapply plus_left. constructor.
-  eapply star_trans. apply step_makeif with (b := false) (v1 := v); auto. congruence.
-  apply push_seq. reflexivity. reflexivity.
-  rewrite <- Kseqlist_app.
-  eapply match_exprstates; eauto.
-  apply S. apply tr_paren_set with (a1 := a2) (t := sd_temp sd); auto.
-  apply tr_expr_monotone with tmp2; eauto. auto. auto.
-(* condition *)
-  exploit tr_top_leftcontext; eauto. clear H9.
-  intros [dst' [sl1 [sl2 [a' [tmp' [P [Q [R S]]]]]]]].
-  inv P. inv H2.
-  (* for value *)
-  exploit tr_simple_rvalue; eauto. intros [SL [TY EV]].
-  subst sl0; simpl Kseqlist. destruct b.
-  econstructor; split.
-  left. eapply plus_left. constructor.
-  eapply star_trans. apply step_makeif with (b := true) (v1 := v); auto. congruence.
-  apply push_seq. reflexivity. reflexivity.
-  rewrite <- Kseqlist_app.
-  eapply match_exprstates; eauto.
-  apply S. econstructor; eauto. apply tr_expr_monotone with tmp2; eauto. auto. auto.
-  econstructor; split.
-  left. eapply plus_left. constructor.
-  eapply star_trans. apply step_makeif with (b := false) (v1 := v); auto. congruence.
-  apply push_seq. reflexivity. reflexivity.
-  rewrite <- Kseqlist_app.
-  eapply match_exprstates; eauto.
-  apply S. econstructor; eauto. apply tr_expr_monotone with tmp3; eauto. auto. auto.
-  (* for effects *)
-  exploit tr_simple_rvalue; eauto. intros [SL [TY EV]].
-  subst sl0; simpl Kseqlist. destruct b.
-  econstructor; split.
-  left. eapply plus_left. constructor.
-  eapply star_trans. apply step_makeif with (b := true) (v1 := v); auto. congruence.
-  apply push_seq.
-  reflexivity. traceEq.
-  rewrite <- Kseqlist_app.
-  econstructor. eauto. apply S.
-    econstructor; eauto. apply tr_expr_monotone with tmp2; eauto.
-    econstructor; eauto.
-  auto. auto.
-  econstructor; split.
-  left. eapply plus_left. constructor.
-  eapply star_trans. apply step_makeif with (b := false) (v1 := v); auto. congruence.
-  apply push_seq.
-  reflexivity. traceEq.
-  rewrite <- Kseqlist_app.
-  econstructor. eauto. apply S.
-    econstructor; eauto. apply tr_expr_monotone with tmp3; eauto.
-    econstructor; eauto.
-  auto. auto.
-  (* for set *)
-  exploit tr_simple_rvalue; eauto. intros [SL [TY EV]].
-  subst sl0; simpl Kseqlist. destruct b.
-  econstructor; split.
-  left. eapply plus_left. constructor.
-  eapply star_trans. apply step_makeif with (b := true) (v1 := v); auto. congruence.
-  apply push_seq.
-  reflexivity. traceEq.
-  rewrite <- Kseqlist_app.
-  econstructor. eauto. apply S.
-    econstructor; eauto. apply tr_expr_monotone with tmp2; eauto.
-    econstructor; eauto.
-  auto. auto.
-  econstructor; split.
-  left. eapply plus_left. constructor.
-  eapply star_trans. apply step_makeif with (b := false) (v1 := v); auto. congruence.
-  apply push_seq.
-  reflexivity. traceEq.
-  rewrite <- Kseqlist_app.
-  econstructor. eauto. apply S.
-    econstructor; eauto. apply tr_expr_monotone with tmp3; eauto.
-    econstructor; eauto.
-  auto. auto.
-(* assign *)
-  exploit tr_top_leftcontext; eauto. clear H12.
-  intros [dst' [sl1 [sl2 [a' [tmp' [P [Q [R S]]]]]]]].
-  inv P. inv H4.
-  (* for effects *)
-  exploit tr_simple_rvalue; eauto. intros [SL2 [TY2 EV2]].
-  exploit tr_simple_lvalue; eauto. intros [SL1 [TY1 EV1]].
-  subst; simpl Kseqlist.
-  econstructor; split.
-  left. eapply plus_left. constructor.
-  apply star_one. eapply step_make_assign; eauto.
-  rewrite <- TY2; eauto. traceEq.
-  econstructor. auto. change sl2 with (nil ++ sl2). apply S.
-  constructor. auto. auto. auto.
-  (* for value *)
-  exploit tr_simple_rvalue; eauto. intros [SL2 [TY2 EV2]].
-  exploit tr_simple_lvalue. eauto.
-    eapply tr_expr_invariant with (le' := PTree.set t0 v' le). eauto.
-    intros. apply PTree.gso. intuition congruence.
-  intros [SL1 [TY1 EV1]].
-  subst; simpl Kseqlist.
-  econstructor; split.
-  left. eapply plus_left. constructor.
-  eapply star_left. constructor. econstructor. eauto. rewrite <- TY2; eauto. 
-  eapply star_left. constructor.
-  apply star_one. eapply step_make_assign; eauto.
-  constructor. apply PTree.gss. simpl. eapply cast_idempotent; eauto. 
-  reflexivity. reflexivity. traceEq.
-  econstructor. auto. apply S.
-  apply tr_val_gen. auto. intros. constructor.
-  rewrite H4; auto. apply PTree.gss.
-  intros. apply PTree.gso. intuition congruence.
-  auto. auto.
-(* assignop *)
-  exploit tr_top_leftcontext; eauto. clear H15.
-  intros [dst' [sl1 [sl2 [a' [tmp' [P [Q [R S]]]]]]]].
-  inv P. inv H6.
-  (* for effects *)
-  exploit tr_simple_lvalue; eauto. intros [SL1 [TY1 EV1]].
-  exploit step_tr_rvalof; eauto. intros [le' [EXEC [EV3 [TY3 INV]]]].
-  exploit tr_simple_lvalue. eauto. eapply tr_expr_invariant with (le := le) (le' := le'). eauto.
-  intros. apply INV. NOTIN. intros [? [? EV1']].
-  exploit tr_simple_rvalue. eauto. eapply tr_expr_invariant with (le := le) (le' := le'). eauto.
-  intros. apply INV. NOTIN. simpl. intros [SL2 [TY2 EV2]].
-  subst; simpl Kseqlist.
-  econstructor; split.
-  left. eapply star_plus_trans. rewrite app_ass. rewrite Kseqlist_app. eexact EXEC.
-  eapply plus_two. simpl. econstructor. eapply step_make_assign; eauto.
-    econstructor. eexact EV3. eexact EV2.
-    rewrite TY3; rewrite <- TY1; rewrite <- TY2; rewrite comp_env_preserved; auto.
-  reflexivity. traceEq.
-  econstructor. auto. change sl2 with (nil ++ sl2). apply S.
-  constructor. auto. auto. auto.
-  (* for value *)
-  exploit tr_simple_lvalue; eauto. intros [SL1 [TY1 EV1]].
-  exploit step_tr_rvalof; eauto. intros [le' [EXEC [EV3 [TY3 INV]]]].
-  exploit tr_simple_lvalue. eauto. eapply tr_expr_invariant with (le := le) (le' := le'). eauto.
-  intros. apply INV. NOTIN. intros [? [? EV1']].
-  exploit tr_simple_rvalue. eauto. eapply tr_expr_invariant with (le := le) (le' := le'). eauto.
-  intros. apply INV. NOTIN. simpl. intros [SL2 [TY2 EV2]].
-  exploit tr_simple_lvalue. eauto.
-    eapply tr_expr_invariant with (le := le) (le' := PTree.set t v4 le'). eauto.
-    intros. rewrite PTree.gso. apply INV. NOTIN. intuition congruence.
-  intros [? [? EV1'']].
-  subst; simpl Kseqlist.
-  econstructor; split.
-  left. rewrite app_ass. rewrite Kseqlist_app.
-  eapply star_plus_trans. eexact EXEC.
-  simpl. eapply plus_four. econstructor. econstructor.
-    econstructor. econstructor. eexact EV3. eexact EV2.
-    rewrite TY3; rewrite <- TY1; rewrite <- TY2; rewrite comp_env_preserved; eauto.
-    eassumption.
-  econstructor. eapply step_make_assign; eauto.
-    constructor. apply PTree.gss. simpl. eapply cast_idempotent; eauto.
-    reflexivity. traceEq.
-  econstructor. auto. apply S.
-  apply tr_val_gen. auto. intros. constructor.
-  rewrite H10; auto. apply PTree.gss.
-  intros. rewrite PTree.gso. apply INV.
-  red; intros; elim H10; auto.
-  intuition congruence.
-  auto. auto.
-(* assignop stuck *)
-  exploit tr_top_leftcontext; eauto. clear H12.
-  intros [dst' [sl1 [sl2 [a' [tmp' [P [Q [R S]]]]]]]].
-  inv P. inv H4.
-  (* for effects *)
-  exploit tr_simple_lvalue; eauto. intros [SL1 [TY1 EV1]].
-  exploit tr_simple_rvalue; eauto. intros [SL2 [TY2 EV2]].
-  exploit step_tr_rvalof; eauto. intros [le' [EXEC [EV3 [TY3 INV]]]].
-  subst; simpl Kseqlist.
-  econstructor; split.
-  right; split. rewrite app_ass. rewrite Kseqlist_app. eexact EXEC.
-  simpl. lia.
-  constructor.
-  (* for value *)
-  exploit tr_simple_lvalue; eauto. intros [SL1 [TY1 EV1]].
-  exploit tr_simple_rvalue; eauto. intros [SL2 [TY2 EV2]].
-  exploit step_tr_rvalof; eauto. intros [le' [EXEC [EV3 [TY3 INV]]]].
-  subst; simpl Kseqlist.
-  econstructor; split.
-  right; split. rewrite app_ass. rewrite Kseqlist_app. eexact EXEC.
-  simpl. lia.
-  constructor.
-(* postincr *)
-  exploit tr_top_leftcontext; eauto. clear H14.
-  intros [dst' [sl1 [sl2 [a' [tmp' [P [Q [R S]]]]]]]].
-  inv P. inv H5.
-  (* for effects *)
-  exploit tr_simple_lvalue; eauto. intros [SL1 [TY1 EV1]].
-  exploit step_tr_rvalof; eauto. intros [le' [EXEC [EV3 [TY3 INV]]]].
-  exploit tr_simple_lvalue. eauto. eapply tr_expr_invariant with (le := le) (le' := le'). eauto.
-  intros. apply INV. NOTIN. intros [? [? EV1']].
-  subst; simpl Kseqlist.
-  econstructor; split.
-  left. rewrite app_ass; rewrite Kseqlist_app.
-  eapply star_plus_trans. eexact EXEC.
-  eapply plus_two. simpl. constructor.
-  eapply step_make_assign; eauto.
-  unfold transl_incrdecr. destruct id; simpl in H2.
-  econstructor. eauto. constructor. rewrite TY3; rewrite <- TY1; rewrite comp_env_preserved. simpl; eauto.
-  econstructor. eauto. constructor. rewrite TY3; rewrite <- TY1; rewrite comp_env_preserved. simpl; eauto.
-  destruct id; auto.
-  reflexivity. traceEq.
-  econstructor. auto. change sl2 with (nil ++ sl2). apply S.
-  constructor. auto. auto. auto.
-  (* for value *)
-  exploit tr_simple_lvalue; eauto. intros [SL1 [TY1 EV1]].
-  exploit tr_simple_lvalue. eauto.
-    eapply tr_expr_invariant with (le' := PTree.set t v1 le). eauto.
-    intros. apply PTree.gso. intuition congruence.
-  intros [SL2 [TY2 EV2]].
-  subst; simpl Kseqlist.
-  econstructor; split.
-  left. eapply plus_four. constructor.
-  eapply step_make_set; eauto.
-  constructor.
-  eapply step_make_assign; eauto.
-  unfold transl_incrdecr. destruct id; simpl in H2.
-  econstructor. constructor. apply PTree.gss. constructor.
-  rewrite comp_env_preserved; simpl; eauto.
-  econstructor. constructor. apply PTree.gss. constructor.
-  rewrite comp_env_preserved; simpl; eauto.
-  destruct id; auto.
-  traceEq.
-  econstructor. auto. apply S.
-  apply tr_val_gen. auto. intros. econstructor; eauto.
-  rewrite H5; auto. apply PTree.gss.
-  intros. apply PTree.gso. intuition congruence.
-  auto. auto.
-(* postincr stuck *)
-  exploit tr_top_leftcontext; eauto. clear H11.
-  intros [dst' [sl1 [sl2 [a' [tmp' [P [Q [R S]]]]]]]].
-  inv P. inv H3.
-  (* for effects *)
-  exploit tr_simple_lvalue; eauto. intros [SL1 [TY1 EV1]].
-  exploit step_tr_rvalof; eauto. intros [le' [EXEC [EV3 [TY3 INV]]]].
-  subst. simpl Kseqlist.
-  econstructor; split.
-  right; split. rewrite app_ass; rewrite Kseqlist_app. eexact EXEC.
-  simpl; lia.
-  constructor.
-  (* for value *)
-  exploit tr_simple_lvalue; eauto. intros [SL1 [TY1 EV1]].
-  subst. simpl Kseqlist.
-  econstructor; split.
-  left. eapply plus_two. constructor. eapply step_make_set; eauto.
-  traceEq.
-  constructor.
-(* comma *)
-  exploit tr_top_leftcontext; eauto. clear H9.
-  intros [dst' [sl1 [sl2 [a' [tmp' [P [Q [R S]]]]]]]].
-  inv P. inv H1.
-  exploit tr_simple_rvalue; eauto. simpl; intro SL1.
-  subst sl0; simpl Kseqlist.
-  econstructor; split.
-  right; split. apply star_refl. simpl. apply plus_lt_compat_r.
-  apply (leftcontext_size _ _ _ H). simpl. lia.
-  econstructor; eauto. apply S.
-  eapply tr_expr_monotone; eauto.
-  auto. auto.
-(* paren *)
-  exploit tr_top_leftcontext; eauto. clear H9.
-  intros [dst' [sl1 [sl2 [a' [tmp' [P [Q [R S]]]]]]]].
-  inv P. inv H2.
-  (* for value *)
-  exploit tr_simple_rvalue; eauto. intros [b [SL1 [TY1 EV1]]].
-  subst sl1; simpl Kseqlist.
-  econstructor; split.
-  left. eapply plus_left. constructor. apply star_one.
-  econstructor. econstructor; eauto. rewrite <- TY1; eauto. traceEq.
-  econstructor; eauto.
-  change sl2 with (final For_val (Etempvar t (Csyntax.typeof r)) ++ sl2). apply S.
-  constructor. auto. intros. constructor. rewrite H2; auto. apply PTree.gss.
-  intros. apply PTree.gso. intuition congruence.
-  auto.
-  (* for effects *)
-  econstructor; split.
-  right; split. apply star_refl. simpl. apply plus_lt_compat_r.
-  apply (leftcontext_size _ _ _ H). simpl. lia.
-  econstructor; eauto.
-  exploit tr_simple_rvalue; eauto. simpl. intros A. subst sl1.
-  apply S. constructor; auto. auto. auto.
-  (* for set *)
-  exploit tr_simple_rvalue; eauto. simpl. intros [b [SL1 [TY1 EV1]]]. subst sl1.
-  simpl Kseqlist.
-  econstructor; split.
-  left. eapply plus_left. constructor. apply star_one. econstructor. econstructor; eauto.
-  rewrite <- TY1; eauto. traceEq.
-  econstructor; eauto.
-  apply S. constructor; auto.
-  intros. constructor. rewrite H2. apply PTree.gss. auto.
-  intros. apply PTree.gso. congruence.
-  auto.
+  Ltac dest_val_effect H dest :=
+    assert (dest = For_val \/ dest = For_effects) as P0; [destruct dest; auto; inv H | inv P0].
 
-(* call *)
-  exploit tr_top_leftcontext; eauto. clear H12.
-  intros [dst' [sl1 [sl2 [a' [tmp' [P [Q [R S]]]]]]]].
-  inv P. inv H5.
-  (* for effects *)
-  exploit tr_simple_rvalue; eauto. intros [SL1 [TY1 EV1]].
-  exploit tr_simple_exprlist; eauto. intros [SL2 EV2].
-  subst. simpl Kseqlist.
-  exploit functions_translated; eauto. intros [tfd [J K]].
-  econstructor; split.
-  left. eapply plus_left. constructor.  apply star_one.
-  econstructor; eauto. rewrite <- TY1; eauto.
-  exploit type_of_fundef_preserved; eauto. congruence.
-  traceEq.
-  constructor; auto. econstructor; eauto.
-  intros. change sl2 with (nil ++ sl2). apply S.
-  constructor. auto. auto.
-  (* for value *)
-  exploit tr_simple_rvalue; eauto. intros [SL1 [TY1 EV1]].
-  exploit tr_simple_exprlist; eauto. intros [SL2 EV2].
-  subst. simpl Kseqlist.
-  exploit functions_translated; eauto. intros [tfd [J K]].
-  econstructor; split.
-  left. eapply plus_left. constructor.  apply star_one.
-  econstructor; eauto. rewrite <- TY1; eauto.
-  exploit type_of_fundef_preserved; eauto. congruence.
-  traceEq.
-  constructor; auto. econstructor; eauto.
-  intros. apply S.
-  destruct dst'; constructor.
-  auto. intros. constructor. rewrite H5; auto. apply PTree.gss.
-  auto. intros. constructor. rewrite H5; auto. apply PTree.gss.
-  intros. apply PTree.gso. intuition congruence.
-  auto.
+  (* expr *)
+  - assert (tr_expr le dest r sl a () tmps).
+   + inv H9; auto. contradiction.
+   + exploit tr_simple_rvalue; eauto. apply soundness3 in H1. intro.
+     apply (soundness1 tmps). iIntros "HA". iDestruct (H1 with "HA") as "HA".
+     iDestruct (H2 with "HA") as "%"; auto. destruct dest.
+     (* for val *)
+      * destruct H3 as (SL1&TY1&EV1). subst sl. iExists _.
+        iSplit; iPureIntro.
+        -- right; split.
+           ++ apply star_refl.
+           ++ destruct r; simpl; (contradiction || lia).
+        -- econstructor; eauto. instantiate (1 := nil). econstructor; auto.
+      (* for effects *)
+      * iClear "HA". subst sl. iExists _.
+        iSplit.
+        -- iPureIntro. right; split.
+           ++ apply star_refl.
+           ++ destruct r; simpl; (contradiction || lia).
+        -- iPureIntro. econstructor; eauto. instantiate (1 := nil). econstructor; auto.
+           simpl. apply soundness2. auto.
+      * inv H10.
 
-(* builtin *)
-  exploit tr_top_leftcontext; eauto. clear H9.
-  intros [dst' [sl1 [sl2 [a' [tmp' [P [Q [R S]]]]]]]].
-  inv P. inv H2.
-  (* for effects *)
-  exploit tr_simple_exprlist; eauto. intros [SL EV].
-  subst. simpl Kseqlist.
-  econstructor; split.
-  left. eapply plus_left. constructor.  apply star_one.
-  econstructor; eauto.
-  eapply external_call_symbols_preserved; eauto. apply senv_preserved.
-  traceEq.
-  econstructor; eauto.
-  change sl2 with (nil ++ sl2). apply S. constructor. simpl; auto. auto.
-  (* for value *)
-  exploit tr_simple_exprlist; eauto. intros [SL EV].
-  subst. simpl Kseqlist.
-  econstructor; split.
-  left. eapply plus_left. constructor. apply star_one.
-  econstructor; eauto.
-  eapply external_call_symbols_preserved; eauto. apply senv_preserved.
-  traceEq.
-  econstructor; eauto.
-  change sl2 with (nil ++ sl2). apply S.
-  apply tr_val_gen. auto. intros. constructor. rewrite H2; auto. simpl. apply PTree.gss.
-  intros; simpl. apply PTree.gso. intuition congruence.
-  auto.
+ (* rval volatile *)
+  - inv H11; simpl in *; auto.
+   + inv H; discriminate.
+   + epose (tr_expr_leftcontext _ _ _ H) as H4. apply soundness3 in H2.
+     apply (soundness1 tmps). iIntros "HA". iDestruct (H2 with "HA") as "HA".
+     iDestruct (H4 with "HA") as (dst'' sl1 sl2 a') "[P [% R]]".
+     simpl. iDestruct "P" as ">P". norm_all.
+     iDestruct (tr_simple_lvalue with "HG") as "[% [% %]]"; eauto. iClear "HG". subst.
+     unfold tr_rvalof. rewrite H3. norm_all. subst.
+     iExists _. iSplit. simpl Kseqlist.
+     * iPureIntro. left. eapply plus_two. constructor. eapply step_make_set; eauto. traceEq.
+     * iConstructor.
+       iIntros "[HA [HB HC]]".
+       iDestruct ("HC" $! (Eval v (Csyntax.typeof l)) with "[]") as "HC"; eauto.
+       iDestruct (locally_set with "[HB] HC") as "[HC HB]"; eauto.
+       iApply (locally_out with "HC"). simpl. destruct dst''.
+       -- iModIntro. iSplit; auto. iIntros. iApply locally_conseq_pure. intros. constructor.
+          eapply H5. simpl. iApply locally_lookup. iFrame.
+       -- iPureIntro. auto.
+       -- iModIntro. iSplit. iFrame. iExists _. iSplitL "HB"; eauto. iIntros.
+          iApply locally_conseq_pure. intros. constructor. eapply H5. simpl. iApply locally_lookup.
+          iFrame. eauto.
+
+ (* seqand true *)
+ - inv H9; simpl in *; auto.
+   + inv H; discriminate.
+   + exploit tr_expr_leftcontext; eauto.
+     intro. apply soundness3 in H2.
+     apply (soundness1 tmps). iIntros "HA". iDestruct (H2 with "HA") as "HA".
+     iDestruct (H3 with "HA") as (dst' sl1 sl2 a') "[P [% R]]". clear H2. clear H3.
+     simpl. iDestruct "P" as ">P".
+     destruct dst'; norm_all; iDestruct (tr_simple_rvalue with "HE") as "[% [% %]]"; eauto; subst;
+       iClear "HE"; iExists _; iSplit;
+         try (iPureIntro; left; simpl Kseqlist;
+              eapply plus_left; [constructor |
+                                 eapply star_trans;
+                                 [ apply step_makeif with (b := true) (v1 := v); auto; congruence|
+                                   apply push_seq | reflexivity] |
+                                 reflexivity]);
+         rewrite <- Kseqlist_app; iConstructor; iIntros "[HA HB]";
+           iDestruct ("HB" $! (Eparen r2 type_bool ty) with "[]") as "HC"; eauto;
+             iApply (locally_out with "HC"); simpl; iModIntro; eauto.
+     iExists _. iExists (sd_temp sd).
+     destruct Pos.eq_dec; auto. contradiction.
+
+ (* seqand false *)
+ - inv H9; simpl in *; auto.
+   + inv H; discriminate.
+   + exploit tr_expr_leftcontext; eauto.
+     intro. apply soundness3 in H2.
+     apply (soundness1 tmps). iIntros "HA". iDestruct (H2 with "HA") as "HA".
+     iDestruct (H3 with "HA") as (dst' sl1 sl2 a') "[P [% R]]". clear H2. clear H3. simpl.
+     destruct dst'; norm_all; iDestruct (tr_simple_rvalue with "HG") as "[% [% %]]"; eauto; subst;
+       iClear "HG"; iExists _; iSplit.
+     * iPureIntro. left. eapply plus_left. simpl Kseqlist. constructor.
+       eapply star_trans. apply step_makeif with (b := false) (v1 := v); auto. congruence.
+       apply star_one. constructor. constructor. reflexivity. reflexivity.
+     * iDestruct (tr_expr_dest with "HI") as ">HG".
+       iDestruct ("R" $! (Eval (Vint Int.zero) ty) with "[]") as "HC"; eauto.
+       iDestruct (locally_set with "HG HC") as "[HC HB]".
+       iConstructor. change sl2 with (nil ++ sl2). iIntros "[HB HA]".
+       iApply (locally_out with "HB"). simpl.
+       iModIntro. iSplitL; auto. iIntros.
+       iApply locally_conseq_pure. intros. constructor. eapply H2.
+       iApply locally_lookup. iFrame.
+     * iPureIntro. left. eapply plus_left. simpl Kseqlist. constructor.
+       apply step_makeif with (b := false) (v1 := v); auto. congruence. reflexivity.
+     * iConstructor. change sl2 with (nil ++ sl2). iIntros "[HA HB]".
+       iDestruct ("HA" $! (Eval (Vint Int.zero) ty) with "[]") as "HA"; eauto.
+       iApply (locally_out with "HA"). simpl. eauto.
+     * iPureIntro. left. eapply plus_left. simpl Kseqlist. constructor.
+       eapply star_trans. apply step_makeif with (b := false) (v1 := v); auto. congruence.
+       apply push_seq. reflexivity. reflexivity.
+     * rewrite <- Kseqlist_app. iConstructor. iIntros "[HB HA]".
+       iDestruct ("HB" $! (Eval (Vint Int.zero) ty) with "[]") as "HB"; eauto.
+       iApply (locally_out with "HB"). simpl. iDestruct (tr_expr_dest with "HA") as ">HA".
+       iFrame. iModIntro. iExists (Econst_int Int.zero ty). iSplitL; eauto.
+       iIntros. iApply locally_simpl. iIntros. iPureIntro. constructor.
+
+ (* seqor true *)
+ - inv H9; simpl in *; auto.
+   + inv H; discriminate.
+   + exploit tr_expr_leftcontext; eauto.
+     intro. apply soundness3 in H2.
+     apply (soundness1 tmps). iIntros "HA". iDestruct (H2 with "HA") as "HA".
+     iDestruct (H3 with "HA") as (dst' sl1 sl2 a') "[P [% R]]". simpl. clear H2. clear H3. simpl.
+     destruct dst'; norm_all; iDestruct (tr_simple_rvalue with "HG") as "[% [% %]]"; eauto; subst;
+       iClear "HG"; iExists _; iSplit.
+       * iPureIntro. left. eapply plus_left. simpl Kseqlist. constructor.
+         eapply star_trans. apply step_makeif with (b := true) (v1 := v); auto. congruence.
+         apply star_one. constructor. constructor. reflexivity. reflexivity.
+       * iDestruct ("R" $! (Eval (Vint Int.one) ty) with "[]") as "HC"; eauto.
+         iDestruct (tr_expr_dest with "HI") as ">HG". iConstructor.
+         change sl2 with (nil ++ sl2). iIntros "[HB HC]".
+         iDestruct (locally_set with "HC HB") as "[HB HC]".
+         change sl2 with (nil ++ sl2). iApply (locally_out with "HB").
+         simpl. iModIntro. iSplitL "HC"; auto. iIntros.
+         iApply locally_conseq_pure. intros. econstructor. eapply H2.
+         iApply locally_lookup. iFrame.
+       * iPureIntro. left. eapply plus_left. simpl Kseqlist. constructor.
+         apply step_makeif with (b := true) (v1 := v); auto. congruence. reflexivity.
+       * iConstructor. change sl2 with (nil ++ sl2). iIntros "[HB HA]".
+         iDestruct ("HB" $! (Eval (Vint Int.one) ty) with "[]") as "HB"; eauto.
+         iApply (locally_out with "HB"). simpl. auto.
+       * iPureIntro. left. eapply plus_left. simpl Kseqlist. constructor.
+         eapply star_trans. apply step_makeif with (b := true) (v1 := v); auto. congruence.
+         apply push_seq. reflexivity. reflexivity.
+       * rewrite <- Kseqlist_app.
+         iDestruct (tr_expr_dest with "HI") as ">HG".
+         iConstructor. iIntros "[HA HB]".
+         iDestruct ("HA" $! (Eval (Vint Int.one) ty) with "[]") as "HA"; eauto.
+         iApply (locally_out with "HA"). simpl. iModIntro. iFrame.
+         iExists (Econst_int Int.one ty). iSplitL; eauto.
+         iIntros. iApply locally_simpl. iIntros. iPureIntro. constructor.
+
+ (* seqor false *)
+ - inv H9; simpl in *; auto.
+   + inv H; discriminate.
+   + exploit tr_expr_leftcontext; eauto.
+     intro. apply soundness3 in H2.
+     apply (soundness1 tmps). iIntros "HA". iDestruct (H2 with "HA") as "HA".
+     iDestruct (H3 with "HA") as (dst' sl1 sl2 a') "[P [% R]]". clear H2. clear H3. simpl.
+     destruct dst'; norm_all; iDestruct (tr_simple_rvalue with "HG") as "[% [% %]]"; eauto;
+       subst; iClear "HG"; iExists _; iSplit.
+     * iPureIntro. left. eapply plus_left. simpl Kseqlist. constructor.
+       eapply star_trans. apply step_makeif with (b := false) (v1 := v); auto. congruence.
+       apply push_seq. constructor. constructor.
+     * rewrite <- Kseqlist_app. iConstructor. iIntros "[HA HB]".
+       iDestruct ("HA" $! (Eparen r2 type_bool ty) with "[]") as "HA"; eauto.
+       iApply (locally_out with "HA").
+       simpl. iModIntro. repeat iExists _. iFrame. eauto.
+     * iPureIntro. left. eapply plus_left. simpl Kseqlist. constructor.
+       eapply star_trans.
+       apply step_makeif with (b := false) (v1 := v); auto. congruence. apply push_seq.
+       reflexivity. reflexivity.
+     * rewrite <- Kseqlist_app. iConstructor. iIntros "[HA HB]".
+       iDestruct ("HA" $! (Eparen r2 type_bool ty) with "[]") as "HA"; eauto.
+       iApply (locally_out with "HA").
+       simpl. iModIntro. iExists _. eauto.
+     * iPureIntro. left. eapply plus_left. simpl Kseqlist. constructor.
+       eapply star_trans. apply step_makeif with (b := false) (v1 := v); auto. congruence.
+       apply push_seq. reflexivity. reflexivity.
+     * rewrite <- Kseqlist_app.
+       iConstructor. iIntros "[HA HB]".
+       iDestruct ("HA" $! (Eparen r2 type_bool ty) with "[]") as "HA"; eauto.
+       iApply (locally_out with "HA").
+       simpl. iModIntro. iExists _. iExists (sd_temp sd).
+       destruct (Pos.eq_dec (sd_temp sd) (sd_temp sd)); auto. contradiction.
+
+ (* condition *)
+ - inv H9; simpl in *; auto.
+   + inv H; discriminate.
+   + exploit tr_expr_leftcontext; eauto.
+     intro. apply soundness3 in H2.
+     apply (soundness1 tmps). iIntros "HA". iDestruct (H2 with "HA") as "HA".
+     iDestruct (H3 with "HA") as (dst' sl1 sl2 a') "[P [% R]]". clear H2. clear H3. simpl.
+     destruct dst'; norm_all.
+     * iDestruct (tr_simple_rvalue with "HG") as "[% [% %]]"; eauto. subst.
+       iClear "HG". destruct b; iExists _; iSplit.
+       -- iPureIntro. left. eapply plus_left. constructor.
+          eapply star_trans. apply step_makeif with (b := true) (v1 := v); auto. congruence.
+          apply push_seq. reflexivity. reflexivity.
+       -- rewrite <- Kseqlist_app. iConstructor. iIntros "[HB HA]".
+          iDestruct ("HB" $! (Eparen r2 ty ty) with "[]") as "HD"; eauto.
+          iApply (locally_out with "HD"). simpl. iModIntro.
+          repeat iExists _. iDestruct "HA" as "[HA _]". iFrame. eauto.
+       -- iPureIntro. left. eapply plus_left. constructor.
+          eapply star_trans. apply step_makeif with (b := false) (v1 := v); auto. congruence.
+          apply push_seq. reflexivity. reflexivity.
+       -- rewrite <- Kseqlist_app. iConstructor. iIntros "[HB HA]".
+          iDestruct ("HB" $! (Eparen r3 ty ty) with "[]") as "HD"; eauto.
+          iApply (locally_out with "HD"). simpl. iModIntro.
+          repeat iExists _. iDestruct "HA" as "[_ HA]". eauto.
+     * iDestruct (tr_simple_rvalue with "HG") as "[% [% %]]"; eauto. subst.
+       iClear "HG". destruct b; iExists _; iSplit.
+       -- iPureIntro. left. eapply plus_left. constructor.
+          eapply star_trans. apply step_makeif with (b := true) (v1 := v); auto. congruence.
+          apply push_seq. reflexivity. traceEq.
+       -- rewrite <- Kseqlist_app. iConstructor. iIntros "[HC [HA HB]]".
+          iDestruct ("HC" $! (Eparen r2 ty ty) with "[]") as "HD"; eauto.
+          iApply (locally_out with "HD"). simpl. iClear "HB". iModIntro.
+          repeat iExists _. iFrame.
+       -- iPureIntro. left. eapply plus_left. constructor.
+          eapply star_trans. apply step_makeif with (b := false) (v1 := v); auto. congruence.
+          apply push_seq. reflexivity. traceEq.
+       -- rewrite <- Kseqlist_app. iConstructor. iIntros "[HC [HA HB]]".
+          iDestruct ("HC" $! (Eparen r3 ty ty) with "[]") as "HD"; eauto.
+          iApply (locally_out with "HD"). simpl. iClear "HA". iModIntro.
+          repeat iExists _. iFrame.
+     * iDestruct (tr_simple_rvalue with "HI") as "[% [% %]]"; eauto. subst.
+       iClear "HI". destruct b; iExists _; iSplit.
+       -- iPureIntro.  left. eapply plus_left. constructor. simpl.
+          eapply star_trans. apply step_makeif with (b := true) (v1 := v); auto. congruence.
+          apply push_seq. reflexivity. traceEq.
+       -- rewrite <- Kseqlist_app. iConstructor. iIntros "[HC [HA HB]]".
+          iDestruct ("HC" $! (Eparen r2 ty ty) with "[]") as "HD"; eauto.
+          iApply (locally_out with "HD"). simpl. iModIntro.
+          iExists _. iExists x5. destruct (Pos.eq_dec x5 (sd_temp sd)).
+          subst. iDestruct "HB" as "[HB _]". iApply tr_expr_abs.
+          iDestruct (tr_expr_dest with "HB") as ">HB". iModIntro.
+          simpl. iDestruct (singleton_neq with "HA HB") as "%". contradiction.
+          iDestruct "HB" as "[HB _]". iFrame.
+       -- iPureIntro. left. eapply plus_left. constructor. simpl.
+          eapply star_trans. apply step_makeif with (b := false) (v1 := v); auto. congruence.
+          apply push_seq. reflexivity. traceEq.
+       -- rewrite <- Kseqlist_app. iConstructor. iIntros "[HC [HA HB]]".
+          iDestruct ("HC" $! (Eparen r3 ty ty) with "[]") as "HD"; eauto.
+          iApply (locally_out with "HD"). simpl. iModIntro. iExists _. iExists x5.
+          destruct (Pos.eq_dec x5 (sd_temp sd)).
+          subst. iDestruct "HB" as "[HB _]". iApply tr_expr_abs.
+          iDestruct (tr_expr_dest with "HB") as ">HB".
+          simpl. iDestruct (singleton_neq with "HA HB") as "%". contradiction.
+          iDestruct "HB" as "[_ HB]". iFrame.
+
+ (* assign *)
+ - inv H12; simpl in *; auto.
+   + inv H; discriminate.
+   + exploit tr_expr_leftcontext; eauto.
+     intro. apply soundness3 in H4.
+     apply (soundness1 tmps). iIntros "HA". iDestruct (H4 with "HA") as "HA".
+     iDestruct (H5 with "HA") as (dst' sl1 sl2 a') "[P [% R]]". clear H4. clear H5.
+     simpl. iDestruct "P" as ">P". destruct dst'; norm_all.
+     * iDestruct (tr_simple_rvalue with "HG") as "[% [% %]]"; eauto.
+       iDestruct (proj1 tr_expr_invariant with "HE") as "HE".
+       iDestruct (locally_set with "[HI] HE") as "[HA HE]"; auto.
+       iDestruct (locally_elim with "HA") as "HA".
+       iDestruct (tr_simple_lvalue with "HA") as "[% [% %]]"; eauto. subst. simpl.
+       iExists _. iSplit.
+       -- iPureIntro. left. eapply plus_left. constructor.
+          eapply star_left. constructor. econstructor. eauto. rewrite <- H8; eauto.
+          eapply star_left. constructor.
+          apply star_one. eapply step_make_assign; eauto.
+          constructor. eapply Maps.PTree.gss. simpl. eapply cast_idempotent; eauto.
+          reflexivity. reflexivity. traceEq.
+       -- iConstructor. iIntros "[HA [_ [HC [HD HE]]]]".
+          iDestruct ("HC" $! (Eval v' (Csyntax.typeof l)) with "[]") as "HB"; eauto.
+          iDestruct (locally_set with "HD HB") as "[HB HC]".
+          change sl2 with (nil ++ sl2). iApply (locally_out with "HB"). simpl.
+          iClear "HA". iClear "HE". iModIntro.
+          iSplitL; eauto. iIntros. iApply locally_conseq_pure. intros. econstructor. eapply H4.
+          iApply locally_lookup. iFrame.
+     * iDestruct (tr_simple_rvalue with "HG") as "[% [% %]]"; eauto.
+       iDestruct (tr_simple_lvalue with "HE") as "[% [% %]]"; eauto. subst. simpl.
+       iExists _. iSplit.
+       -- iPureIntro. left. eapply plus_left. constructor.
+          apply star_one. eapply step_make_assign; eauto.
+          rewrite <- H7; eauto. traceEq.
+       -- iConstructor. change sl2 with (nil ++ sl2). iIntros "[HA [HB HC]]".
+          iDestruct ("HC" $! (Eval v' (Csyntax.typeof l)) with "[]") as "HC"; eauto.
+          iApply (locally_out with "HC"). simpl. eauto.
+     * iDestruct (tr_simple_rvalue with "HG") as "[% [% %]]"; eauto.
+       iDestruct (proj1 tr_expr_invariant with "HE") as "HA".
+       iDestruct (locally_set with "[HI] HA") as "[HA HC]"; auto.
+       iDestruct (locally_elim with "HA") as "HA".
+       iDestruct (tr_simple_lvalue with "HA") as "[% [% %]]"; eauto. subst. simpl.
+       iExists _. iSplit.
+       -- iPureIntro. left. eapply plus_left. constructor.
+          eapply star_left. constructor. econstructor. eauto. rewrite <- H8; eauto.
+          eapply star_left. constructor.
+          apply star_one. eapply step_make_assign; eauto.
+          constructor. eapply Maps.PTree.gss. simpl. eapply cast_idempotent; eauto.
+          reflexivity. reflexivity. traceEq.
+       -- iConstructor. iIntros "[HA [HB [HC [HD HE]]]]".
+          iDestruct ("HC" $! (Eval v' (Csyntax.typeof l)) with "[]") as "HC"; eauto.
+          iDestruct (locally_set with "HD HC") as "[HC HD]".
+          change sl2 with (nil ++ sl2). iApply (locally_out with "HC"). simpl.
+          iClear "HA". iClear "HE". iModIntro. iFrame. repeat iExists _.
+          iSplitL; eauto. iIntros. iApply locally_conseq_pure. intros. econstructor. eapply H4.
+          iApply locally_lookup. iFrame.
+          iPureIntro. split; eauto.
+
+ (* assignop *)
+ - inv H15; simpl in *; auto.
+   + inv H; discriminate.
+   + exploit tr_expr_leftcontext; eauto.
+     intro. apply soundness3 in H6.
+     apply (soundness1 tmps). iIntros "HA". iDestruct (H6 with "HA") as "HA".
+     iDestruct (H7 with "HA") as (dst' sl1 sl2 a') "[P [% R]]". clear H6. clear H7.
+     simpl. iDestruct "P" as ">P". destruct dst'; norm_all.
+     * unfold tr_rvalof. destruct (type_is_volatile (Csyntax.typeof l)) eqn:?; norm_all.
+       -- iDestruct (tr_simple_lvalue with "HG") as "[% [% %]]"; eauto.
+          iDestruct (proj1 tr_expr_invariant with "HI") as "HB".
+          (* iDestruct (locally_set with "[HK] HB") as "[HB HC]"; eauto. *)
+          iDestruct (locally_set with "[HT] HB") as "[HB HD]"; eauto.
+          iDestruct (locally_elim with "HB") as "HB".
+          iDestruct (tr_simple_rvalue with "HB") as "[% [% %]]"; eauto. subst.
+          iDestruct (proj1 tr_expr_invariant with "HG") as "HA".
+          iDestruct (locally_set with "[HD] HA") as "[HA HD]"; eauto.
+          iDestruct (locally_set with "[HM] HA") as "[HA HC]"; eauto.
+          iDestruct (locally_elim with "HA") as "HA".
+          iDestruct (tr_simple_lvalue with "HA") as "[% [% %]]"; eauto.
+          iExists _. iSplit.
+          ++ iPureIntro.
+             left. rewrite app_ass. rewrite Kseqlist_app.
+             eapply star_plus_trans. eapply star_two.
+             econstructor. eapply step_make_set; eauto. traceEq.
+             simpl. eapply plus_four. econstructor. econstructor.
+             econstructor. econstructor. constructor. apply Maps.PTree.gss.
+             eauto. rewrite <- H17. rewrite comp_env_preserved. simpl. eauto. eassumption.
+             econstructor. eapply step_make_assign; eauto.
+             econstructor. apply Maps.PTree.gss. simpl. eapply cast_idempotent; eauto.
+             reflexivity. traceEq.
+          ++ iClear "HB". iDestruct ("R" $! (Eval v4 (Csyntax.typeof l)) with "[]") as "HB"; eauto.
+             iDestruct (locally_set with "HD HB") as "[HB HD]".
+             iDestruct (locally_set with "HC HB") as "[HB HC]".
+             iClear "HA". iClear "HD". iConstructor. iIntros "[_ [HA HB]]".
+             change sl2 with (nil ++ sl2).
+             iApply (locally_out with "HA"). simpl. iModIntro. iSplitL "HB"; eauto.
+             iIntros "*". iApply locally_conseq_pure. intros. econstructor. apply H9.
+             iApply locally_lookup. iFrame.
+       -- iDestruct (tr_simple_lvalue with "HG") as "[% [% %]]"; eauto.
+          iDestruct (proj1 tr_expr_invariant with "HG") as "HA".
+          iDestruct (locally_set with "[HM] HA") as "[HA HC]"; auto.
+          iDestruct (locally_elim with "HA") as "HA".
+          iDestruct (tr_simple_lvalue with "HA") as "[% [% %]]"; eauto.
+          iDestruct (tr_simple_rvalue with "HI") as "[% [% %]]"; eauto.
+          iDestruct (proj1 tr_expr_invariant with "HI") as "HB".
+          iDestruct (locally_set with "HC HB") as "[HB HC]".
+          iDestruct (locally_elim with "HB") as "HB".
+          iDestruct (tr_simple_rvalue with "HB") as "[% [% %]]"; eauto. subst. simpl.
+          exploit deref_loc_translated; eauto. intros. unfold chunk_for_volatile_type in H6.
+          rewrite Heqb0 in H6. destruct H6.
+          iExists _. iSplit.
+          ++ iPureIntro.
+             left. eapply star_plus_trans. apply star_refl.
+             simpl. eapply plus_four. econstructor. econstructor.
+             econstructor. econstructor. eapply eval_Elvalue; eauto. rewrite <- H12. eauto.
+             eauto. rewrite <- H12. rewrite <- H23. rewrite comp_env_preserved. eauto.
+             eassumption. econstructor. eapply step_make_assign; eauto.
+             constructor. apply Maps.PTree.gss. simpl. eapply cast_idempotent; eauto.
+             reflexivity. traceEq.
+          ++ iClear "HE". instantiate (1 := v4). iClear "HA". iClear "HB".
+             iConstructor. iIntros "[HA HB]".
+             iDestruct ("HA" $! (Eval v4 (Csyntax.typeof l)) with "[]") as "HA"; eauto.
+             iDestruct (locally_set with "[HB] HA") as "[HA HB]"; eauto.
+             change sl2 with (nil ++ sl2).
+             iApply (locally_out with "HA").
+             simpl. iModIntro. iSplitL "HB"; eauto.
+             iIntros "*". iApply locally_conseq_pure. intros. econstructor. apply H8.
+             iApply locally_lookup. iFrame.
+     * unfold tr_rvalof. destruct (type_is_volatile (Csyntax.typeof l)) eqn:?; norm_all.
+       -- iDestruct (tr_simple_lvalue with "HE") as "[% [% %]]"; eauto.
+          iDestruct (proj1 tr_expr_invariant with "HE") as "HA".
+          iDestruct (locally_set with "[HL] HA") as "[HA HC]"; eauto.
+          iDestruct (locally_elim with "HA") as "HA".
+          iDestruct (tr_simple_lvalue with "HA") as "[% [% %]]"; eauto.
+          iDestruct (tr_simple_rvalue with "HG") as "[% [% %]]"; eauto.
+          iDestruct (proj1 tr_expr_invariant with "HG") as "HB".
+          iDestruct (locally_set with "[HC] HB") as "[HB HC]"; eauto.
+          iDestruct (locally_elim with "HB") as "HB".
+          iDestruct (tr_simple_rvalue with "HB") as "[% [% %]]"; eauto. subst. simpl.
+          iExists _. iSplit.
+          ++ iPureIntro.
+             left. eapply star_plus_trans. eapply star_two. econstructor.
+             eapply step_make_set; eauto. traceEq.
+             eapply plus_two. simpl. econstructor. eapply step_make_assign; eauto.
+             econstructor. constructor. apply Maps.PTree.gss. eauto.
+             rewrite comp_env_preserved. simpl. rewrite <- H22. auto. reflexivity. traceEq.
+          ++ iClear "HA". iClear "HB".
+             iDestruct ("R" $! (Eval v4 (Csyntax.typeof l)) with "[]") as "HA"; eauto.
+             iDestruct (locally_set with "HC HA") as "[HA HC]". iClear "HC".
+             iConstructor. iIntros "HA". change sl2 with (nil ++ sl2).
+             iApply (locally_out with "HA"). simpl. iModIntro. auto.
+       -- iDestruct (tr_simple_lvalue with "HE") as "[% [% %]]"; eauto.
+          iDestruct (tr_simple_rvalue with "HG") as "[% [% %]]"; eauto.
+          exploit deref_loc_translated; eauto. intros. unfold chunk_for_volatile_type in H18.
+          rewrite Heqb0 in H18. destruct H18. subst. simpl.
+          iExists _. iSplit.
+          ++ iPureIntro.
+             left. eapply star_plus_trans. apply star_refl.
+             eapply plus_two. simpl. econstructor. eapply step_make_assign; eauto.
+             econstructor. eapply eval_Elvalue; eauto. rewrite <- H11. eauto. eauto.
+             rewrite <- H11. rewrite <- H15. rewrite comp_env_preserved. auto.
+             reflexivity. traceEq.
+          ++ iClear "HE". iClear "HG". iConstructor. iIntros "HC".
+             iDestruct ("HC" $! (Eval v4 (Csyntax.typeof l)) with "[]") as "HC"; eauto.
+             change sl2 with (nil ++ sl2).
+             iApply (locally_out with "HC"). simpl. iModIntro. auto.
+     * unfold tr_rvalof. destruct (type_is_volatile (Csyntax.typeof l)) eqn:?; norm_all.
+       -- iDestruct (tr_simple_lvalue with "HG") as "[% [% %]]"; eauto.
+          iDestruct (proj1 tr_expr_invariant with "HI") as "HB".
+          iDestruct (locally_set with "[HT] HB") as "[HB HC]"; eauto.
+          iDestruct (locally_elim with "HB") as "HB".
+          iDestruct (tr_simple_rvalue with "HB") as "[% [% %]]"; eauto. subst.
+          iDestruct (proj1 tr_expr_invariant with "HG") as "HA".
+          iDestruct (locally_set with "[HC] HA") as "[HA HC]"; eauto.
+          iDestruct (locally_set with "[HM] HA") as "[HA HD]"; eauto.
+          iDestruct (locally_elim with "HA") as "HA".
+          iDestruct (tr_simple_lvalue with "HA") as "[% [% %]]"; eauto.
+          iExists _. iSplit.
+          ++ iPureIntro.
+             left. rewrite app_ass. rewrite Kseqlist_app.
+             eapply star_plus_trans. eapply star_two.
+             econstructor. eapply step_make_set; eauto. traceEq.
+             simpl. eapply plus_four. econstructor. econstructor.
+             econstructor. econstructor. constructor. apply Maps.PTree.gss.
+             eauto. rewrite <- H17. rewrite comp_env_preserved. simpl. eauto. eassumption.
+             econstructor. eapply step_make_assign; eauto.
+             econstructor. apply Maps.PTree.gss. simpl. eapply cast_idempotent; eauto.
+             reflexivity. traceEq.
+          ++ iClear "HA". iClear "HB".
+             iDestruct ("R" $! (Eval v4 (Csyntax.typeof l)) with "[]") as "HA"; eauto.
+             iDestruct (locally_set with "[HC] HA") as "[HA HC]"; eauto.
+             iDestruct (locally_set with "[HD] HA") as "[HA HD]"; eauto.
+             iClear "HC". iConstructor. iIntros "[HF [HA HB]]". change sl2 with (nil ++ sl2).
+             iApply (locally_out with "HA"). simpl. iModIntro. iFrame. iExists _.
+             iSplitL "HB"; eauto. iIntros "*". iApply locally_conseq_pure. intros. econstructor.
+             apply H9. iApply locally_lookup. iFrame. eauto.
+       -- iDestruct (tr_simple_lvalue with "HG") as "[% [% %]]"; eauto.
+          iDestruct (proj1 tr_expr_invariant with "HG") as "HA".
+          iDestruct (locally_set with "[HM] HA") as "[HA HC]"; auto.
+          iDestruct (locally_elim with "HA") as "HA".
+          iDestruct (tr_simple_lvalue with "HA") as "[% [% %]]"; eauto.
+          iDestruct (tr_simple_rvalue with "HI") as "[% [% %]]"; eauto.
+          iDestruct (proj1 tr_expr_invariant with "HI") as "HB".
+          iDestruct (locally_set with "HC HB") as "[HB HC]".
+          iDestruct (locally_elim with "HB") as "HB".
+          iDestruct (tr_simple_rvalue with "HB") as "[% [% %]]"; eauto. subst. simpl.
+          exploit deref_loc_translated; eauto. intros. unfold chunk_for_volatile_type in H6.
+          rewrite Heqb0 in H6. destruct H6.
+          iExists _. iSplit.
+          ++ iPureIntro.
+             left. eapply star_plus_trans. apply star_refl.
+             simpl. eapply plus_four. econstructor. econstructor.
+             econstructor. econstructor. eapply eval_Elvalue; eauto. rewrite <- H12. eauto.
+             eauto. rewrite <- H12. rewrite <- H23. rewrite comp_env_preserved. eauto.
+             eassumption. econstructor. eapply step_make_assign; eauto.
+             constructor. apply Maps.PTree.gss. simpl. eapply cast_idempotent; eauto.
+             reflexivity. traceEq.
+          ++ instantiate (1 := v4).
+             iDestruct ("R" $! (Eval v4 (Csyntax.typeof l)) with "[]") as "R"; eauto.
+             iDestruct (locally_set with "[HC] R") as "[R HC]"; eauto.
+             iClear "HA". iClear "HB".
+             iConstructor. iIntros "[HA [HB HC]]". change sl2 with (nil ++ sl2).
+             iApply (locally_out with "HB").
+             simpl. iModIntro. iFrame. iExists _. iSplitL "HC"; eauto.
+             iIntros "*". iApply locally_conseq_pure. intros. econstructor. apply H8.
+             iApply locally_lookup. iFrame. eauto.
+
+ (* assignop stuck *)
+ - inv H12; simpl in *; auto.
+   + inv H; discriminate.
+   + exploit tr_expr_leftcontext; eauto.
+     intro. apply soundness3 in H4.
+     apply (soundness1 tmps). iIntros "HA". iDestruct (H4 with "HA") as "HA".
+     iDestruct (H5 with "HA") as (dst' sl1 sl2 a') "[P [% R]]". clear H4. clear H5.
+     simpl. iDestruct "P" as ">P". destruct dst'; norm_all.
+     * iDestruct (tr_simple_lvalue with "HG") as "[% [% %]]"; eauto.
+       iDestruct (tr_simple_rvalue with "HI") as "[% [% %]]"; eauto.
+       iDestruct (step_tr_rvalof with "HK") as (le') "[% [% %]]"; eauto.
+       subst. simpl.
+       iExists _. iSplit.
+       ++ iPureIntro.
+          right; split. rewrite app_ass. rewrite Kseqlist_app. eexact H15. lia.
+       ++ iPureIntro. econstructor.
+     * iDestruct (tr_simple_lvalue with "HE") as "[% [% %]]"; eauto.
+       iDestruct (tr_simple_rvalue with "HG") as "[% [% %]]"; eauto.
+       iDestruct (step_tr_rvalof with "HI") as (le') "[% [% %]]"; eauto.
+       subst. simpl. iExists _. iSplit.
+       ++ iPureIntro. right; split. rewrite app_ass. rewrite Kseqlist_app. eexact H14. lia.
+       ++ iPureIntro. econstructor.
+     * iDestruct (tr_simple_lvalue with "HG") as "[% [% %]]"; eauto.
+       iDestruct (tr_simple_rvalue with "HI") as "[% [% %]]"; eauto.
+       iDestruct (step_tr_rvalof with "HK") as (le') "[% [% %]]"; eauto.
+       subst. simpl. iExists _. iSplit.
+       ++ iPureIntro. right; split. rewrite app_ass. rewrite Kseqlist_app. eexact H15. lia.
+       ++ iPureIntro. econstructor.
+
+  (* postincr *)
+ - inv H14; simpl in *; auto.
+   + inv H; discriminate.
+   + exploit tr_expr_leftcontext; eauto. intro. apply soundness3 in H5.
+     apply (soundness1 tmps). iIntros "HA". iDestruct (H5 with "HA") as "HA".
+     iDestruct (H6 with "HA") as (dst' sl1 sl2 a') "[P [% R]]". clear H5. clear H6.
+     simpl. iDestruct "P" as ">P". norm_all. destruct dst'; norm_all.
+     * iDestruct (tr_simple_lvalue with "HE") as "[% [% %]]"; eauto.
+       iDestruct (proj1 tr_expr_invariant with "HE") as "HA".
+       iDestruct (locally_set with "[HI] HA") as "[HA HB]"; auto.
+       iDestruct (locally_elim with "HA") as "HA".
+       iDestruct (tr_simple_lvalue with "HA") as "[% [% %]]"; eauto.
+       subst. simpl. iExists _. iSplit.
+       -- iPureIntro. left. eapply plus_four. constructor.
+          eapply step_make_set; eauto. constructor. eapply step_make_assign; eauto.
+          unfold transl_incrdecr. destruct id; simpl in H2.
+          econstructor. constructor. apply Maps.PTree.gss. constructor.
+          rewrite comp_env_preserved; simpl; eauto.
+          econstructor. constructor. apply Maps.PTree.gss. constructor.
+          rewrite comp_env_preserved; simpl; eauto.
+          destruct id; auto. traceEq.
+       -- iClear "HA". iClear "HG". iConstructor. iIntros "[HA HB]".
+          iDestruct ("HA" $! (Eval v1 (Csyntax.typeof l)) with "[]") as "HA"; eauto.
+          iDestruct (locally_set with "HB HA") as "[HA HB]". change sl2 with (nil ++ sl2).
+          iApply (locally_out with "HA"). simpl. iModIntro. iSplitL "HB"; eauto.
+          iIntros "*". iApply locally_conseq_pure. intros. econstructor. apply H5.
+          iApply locally_lookup. iFrame.
+     * iDestruct (tr_simple_lvalue with "HE") as "[% [% %]]"; eauto.
+       unfold tr_rvalof. destruct (type_is_volatile (Csyntax.typeof l)) eqn:?; norm_all.
+       -- iDestruct (proj1 tr_expr_invariant with "HE") as "HA".
+          iDestruct (locally_set with "[HM] HA") as "[HA HB]"; eauto.
+          iDestruct (locally_elim with "HA") as "HA".
+          iDestruct (tr_simple_lvalue with "HA") as "[% [% %]]"; eauto.
+          subst. iExists _. iSplit.
+          ++ iPureIntro. left. rewrite app_ass; rewrite Kseqlist_app. eapply star_plus_trans.
+             eapply star_two. econstructor. eapply step_make_set; eauto. traceEq.
+             eapply plus_two. simpl. constructor. eapply step_make_assign; eauto.
+             unfold transl_incrdecr. destruct id; simpl in H2.
+             econstructor. constructor. apply Maps.PTree.gss. econstructor.
+             rewrite comp_env_preserved. simpl. eauto.
+             econstructor. econstructor. apply Maps.PTree.gss. econstructor.
+             rewrite comp_env_preserved. simpl; eauto.
+             destruct id; auto. reflexivity. traceEq.
+          ++ iClear "HA". iDestruct ("R" $! (Eval v1 (Csyntax.typeof l)) with "[]") as "HA"; eauto.
+             iDestruct (locally_set with "HB HA") as "[HA HB]". iClear "HB".
+             iConstructor. iIntros "HA". change sl2 with (nil ++ sl2).
+             iApply (locally_out with "HA"). simpl. iModIntro. eauto.
+       -- iDestruct (tr_simple_lvalue with "HE") as "[% [% %]]"; eauto.
+          exploit deref_loc_translated; eauto. intros. unfold chunk_for_volatile_type in H17.
+          rewrite Heqb0 in H17. destruct H17. subst. iExists _. iSplit.
+          ++ iPureIntro. left. rewrite app_ass; rewrite Kseqlist_app.
+             eapply star_plus_trans. eapply star_refl.
+             eapply plus_two. simpl. constructor.
+             eapply step_make_assign; eauto.
+             unfold transl_incrdecr. destruct id; simpl in H2.
+             econstructor. econstructor; eauto. rewrite <- H8. eauto. econstructor.
+             rewrite comp_env_preserved. simpl. rewrite <- H8. eauto.
+             econstructor. econstructor. eauto. rewrite <- H8. eauto. econstructor.
+             rewrite comp_env_preserved. simpl. rewrite <- H8. eauto.
+             unfold transl_incrdecr. destruct id; simpl in H2. eauto. eauto. reflexivity.
+             traceEq.
+          ++ iConstructor. iIntros "[HA HB]".
+             iDestruct ("HB" $! (Eval v1 (Csyntax.typeof l)) with "[]") as "HB"; eauto.
+             change sl2 with (nil ++ sl2). iApply (locally_out with "HB"). simpl. eauto.
+     * iDestruct (tr_simple_lvalue with "HE") as "[% [% %]]"; eauto.
+       iDestruct (proj1 tr_expr_invariant with "HE") as "HA".
+       iDestruct (locally_set with "[HI] HA") as "[HA HB]"; auto.
+       iDestruct (locally_elim with "HA") as "HA".
+       iDestruct (tr_simple_lvalue with "HA") as "[% [% %]]"; eauto.
+       subst. simpl. iExists _. iSplit.
+       -- iPureIntro.
+          left. eapply plus_four. constructor.
+          eapply step_make_set; eauto. constructor.
+          eapply step_make_assign; eauto.
+          unfold transl_incrdecr. destruct id; simpl in H2.
+          econstructor. constructor. apply Maps.PTree.gss. constructor.
+          rewrite comp_env_preserved; simpl; eauto.
+          econstructor. constructor. apply Maps.PTree.gss. constructor.
+          rewrite comp_env_preserved; simpl; eauto.
+          destruct id; auto. traceEq.
+       -- iClear "HA". iConstructor. iIntros "[HB [HA HC]]".
+          iDestruct ("HA" $! (Eval v1 (Csyntax.typeof l)) with "[]") as "HA"; eauto.
+          iDestruct (locally_set with "HC HA") as "[HA HC]".
+          change sl2 with (nil ++ sl2).
+          iApply (locally_out with "HA"). simpl. iModIntro. iFrame. iExists _. iSplitL "HC"; eauto.
+          iIntros "*". iApply locally_conseq_pure. intros. econstructor. apply H5.
+          iApply locally_lookup. iFrame. eauto.
+
+ (* postincr stuck *)
+ - inv H11; simpl in *; auto.
+   + inv H; discriminate.
+   + exploit tr_expr_leftcontext; eauto.
+     intro. apply soundness3 in H3.
+     apply (soundness1 tmps). iIntros "HA". iDestruct (H3 with "HA") as "HA".
+     iDestruct (H4 with "HA") as (dst' sl1 sl2 a') "[P [% R]]". clear H3. clear H4.
+     simpl. iDestruct "P" as ">P"; norm_all. destruct dst'; norm_all.
+     * iDestruct (tr_simple_lvalue with "HE") as "[% [% %]]"; eauto.
+       subst. simpl. iExists _. iSplit.
+       -- iPureIntro. left. eapply plus_two. constructor. eapply step_make_set; eauto. traceEq.
+       -- iPureIntro. econstructor.
+     * iDestruct (tr_simple_lvalue with "HE") as "[% [% %]]"; eauto.
+       iDestruct (step_tr_rvalof with "HG") as (le') "[% [% %]]"; eauto. subst.
+       iExists _. iSplit.
+       -- iPureIntro. right; split. simpl. rewrite app_ass; rewrite Kseqlist_app. eexact H8. lia.
+       -- iPureIntro. econstructor.
+     * iDestruct (tr_simple_lvalue with "HE") as "[% [% %]]"; eauto.
+       subst. simpl. iExists _. iSplit.
+       -- iPureIntro. left. eapply plus_two. constructor. eapply step_make_set; eauto. traceEq.
+       -- iPureIntro. econstructor.
+
+ (* comma *)
+ - inv H9; simpl in *; auto.
+   + inv H; discriminate.
+   + exploit tr_expr_leftcontext; eauto.
+     intro. apply soundness3 in H1.
+     apply (soundness1 tmps). iIntros "HA". iDestruct (H1 with "HA") as "HA".
+     iDestruct (H2 with "HA") as (dst' sl1 sl2 a') "[P [% R]]". clear H1. clear H2.
+     simpl. iDestruct "P" as (sl0 a2 sl3) ">P"; norm_all.
+     iDestruct (tr_simple_rvalue with "HE") as "%"; eauto. iClear "HE".
+     iExists _. iSplit.
+     * iPureIntro. right; split. apply star_refl. apply plus_lt_compat_r.
+        apply (leftcontext_size _ _ _ H). simpl. omega.
+     * iConstructor. iIntros "[HB HD]". iDestruct ("HD" $! r2 with "[]") as "HD"; eauto.
+       subst. iApply (locally_out with "HD"). simpl. iFrame.
+
+ (* paren *)
+ - inv H9; simpl in *; auto.
+   + inv H; discriminate.
+   + exploit tr_expr_leftcontext; eauto.
+     intro. apply soundness3 in H2.
+     apply (soundness1 tmps). iIntros "HA". iDestruct (H2 with "HA") as "HA".
+     iDestruct (H3 with "HA") as (dst' sl1 sl2 a') "[P [% R]]". clear H2. clear H3.
+     simpl. iDestruct "P" as ">P". destruct dst'; norm_all.
+     * iDestruct (tr_simple_rvalue with "HE") as (b) "[% [% %]]"; eauto. subst; simpl.
+       iExists _. iSplit.
+       -- iPureIntro. left. eapply plus_left. constructor. apply star_one. econstructor.
+          econstructor; eauto. rewrite <- H5; eauto. traceEq.
+       -- iDestruct ("R" $! (Eval v ty) with "[]") as "R"; eauto.
+          iDestruct (tr_expr_dest with "HE") as ">HA".
+          iDestruct (locally_set with "HA R") as "[R HA]".
+          iConstructor. iIntros "[HA HB]". change sl2 with (nil ++ sl2).
+          iApply (locally_out with "HA"). simpl. iModIntro. iSplitL "HB"; eauto.
+          iIntros "*". iApply locally_conseq_pure. intros. econstructor. apply H2.
+          iApply locally_lookup. iFrame.
+     * iDestruct (tr_simple_rvalue with "P") as "%"; eauto. subst; simpl.
+       iExists _. iSplit.
+       -- iPureIntro. right; split. apply star_refl. simpl. apply plus_lt_compat_r.
+          apply (leftcontext_size _ _ _ H). simpl. lia.
+       -- iConstructor. iIntros "[HA HB]".
+          iDestruct ("HB" $! (Eval v ty) with "[]") as "HC"; eauto.
+          change sl2 with (nil ++ sl2).
+          iApply (locally_out with "HC"). simpl. eauto.
+     * destruct (Pos.eq_dec x0 (sd_temp sd)); norm_all.
+       -- subst.
+          iDestruct (tr_simple_rvalue with "P") as (b) "[% [% %]]"; eauto. subst; simpl.
+          iExists _. iSplit.
+          ++ iPureIntro. left. eapply plus_left. constructor. apply star_one. econstructor.
+             econstructor; eauto. rewrite <- H3; eauto. traceEq.
+          ++ iDestruct ("R" $! (Eval v ty) with "[]") as "R"; eauto.
+             iDestruct (tr_expr_dest with "P") as ">HA".
+             iDestruct (locally_set with "HA R") as "[R HA]".
+             iConstructor. iIntros "[HA HB]". change sl2 with (nil ++ sl2).
+             iApply (locally_out with "HA"). simpl. iModIntro. iSplit; iFrame. iExists _.
+             iSplitL; auto. iIntros "*". iApply locally_conseq_pure. intros. econstructor. apply H2.
+             iApply locally_lookup. iFrame. eauto.
+       -- iDestruct (tr_simple_rvalue with "HE") as (b) "[% [% %]]"; eauto. subst; simpl.
+          iExists _. iSplit.
+          ++ iPureIntro. left. eapply plus_left. constructor. apply star_one. econstructor.
+             econstructor; eauto. rewrite <- H3; eauto. traceEq.
+          ++ iDestruct ("R" $! (Eval v ty) with "[]") as "R"; eauto.
+             iDestruct (tr_expr_dest with "HE") as ">HA".
+             iDestruct (locally_set with "HA R") as "[R HA]".
+             iConstructor. iIntros "[HA [HB HC]]". change sl2 with (nil ++ sl2).
+             iApply (locally_out with "HB"). simpl. iModIntro. iSplit; iFrame. iExists _.
+             iSplitL "HC"; auto. iIntros "*". iApply locally_conseq_pure. intros. econstructor.
+             apply H2. iApply locally_lookup. iFrame. eauto.
+
+ (* call *)
+ - inv H12; simpl in *; auto.
+   + inv H; discriminate.
+   + exploit tr_expr_leftcontext; eauto.
+     intro. apply soundness3 in H5.
+     apply (soundness1 tmps). iIntros "HA". iDestruct (H5 with "HA") as "HA".
+     iDestruct (H6 with "HA") as (dst' sl1 sl2 a') "[P [% R]]". clear H5. clear H6.
+     simpl. iDestruct "P" as ">P". destruct dst'; norm_all.
+     * iDestruct (tr_simple_rvalue with "HI") as "[% [% %]]"; eauto.
+       iDestruct (tr_simple_exprlist with "HK []") as "[% %]"; eauto.
+       subst. simpl. exploit functions_translated; eauto. intros [tfd [J K]].
+       iExists _. iSplit.
+       -- iPureIntro. left. eapply plus_left. constructor. apply star_one.
+          econstructor; eauto. rewrite <- H9; eauto.
+          exploit type_of_fundef_preserved; eauto. congruence. traceEq.
+       -- iClear "HI HK HE". iStopProof. apply instance_heap. intros.
+          econstructor; eauto. econstructor; eauto. intros. econstructor.
+          apply soundness2. apply soundness3 in H5. iIntros "HA".
+          iDestruct (H5 with "HA") as "[HA HD]".
+          iDestruct ("HD" $! (Eval v ty) with "[]") as "HD"; eauto.
+          change sl2 with (nil ++ sl2). unfold set_opttemp.
+          iDestruct (locally_set with "[HA] HD") as "[HD HA]"; auto.
+          iApply (locally_out with "HD"). iModIntro. iSplitL "HA".
+          iIntros. iApply locally_conseq_pure. intros. econstructor. eapply H6.
+          iApply locally_lookup. iFrame. eauto.
+     * iDestruct (tr_simple_rvalue with "HE") as "[% [% %]]"; eauto.
+       iDestruct (tr_simple_exprlist with "HG []") as "[% %]"; eauto.
+       subst. simpl. exploit functions_translated; eauto. intros [tfd [J K]].
+       iExists _. iSplit.
+       -- iPureIntro. left. eapply plus_left. constructor. apply star_one.
+          econstructor; eauto. rewrite <- H8; eauto.
+          exploit type_of_fundef_preserved; eauto. congruence. traceEq.
+       -- iStopProof. apply instance_heap. intros.
+          econstructor; eauto. econstructor; eauto. intros. econstructor.
+          apply soundness2. apply soundness3 in H5. iIntros "HA".
+          iDestruct (H5 with "HA") as "[HA [HB HC]]".
+          iDestruct ("HC" $! (Eval v ty) with "[]") as "HD"; eauto.
+          change sl2 with (nil ++ sl2). unfold set_opttemp.
+          iApply (locally_out with "HD"). eauto.
+     * iDestruct (tr_simple_rvalue with "HI") as "[% [% %]]"; eauto.
+       iDestruct (tr_simple_exprlist with "HK []") as "[% %]"; eauto.
+       subst. simpl. exploit functions_translated; eauto. intros [tfd [J K]].
+       iExists _. iSplit.
+       -- iPureIntro. left. eapply plus_left. constructor. apply star_one.
+          econstructor; eauto. rewrite <- H9; eauto.
+          exploit type_of_fundef_preserved; eauto. congruence. traceEq.
+       -- iClear "HI HK". iStopProof. apply instance_heap. intros.
+          econstructor; eauto. econstructor; eauto. intros. econstructor.
+          apply soundness2. apply soundness3 in H5. iIntros "HA".
+          iDestruct (H5 with "HA") as "[HA [HB HD]]".
+          iDestruct ("HD" $! (Eval v ty) with "[]") as "HD"; eauto.
+          change sl2 with (nil ++ sl2). unfold set_opttemp.
+          iDestruct (locally_set with "[HB] HD") as "[HD HB]"; auto.
+          iApply (locally_out with "HD"). iModIntro. iSplit; iFrame. iExists _. iSplitL "HB".
+          iIntros. iApply locally_conseq_pure. intros. econstructor. eapply H6.
+          iApply locally_lookup. iFrame. eauto.
+
+ (* ebuiltin *)
+ - inv H9; simpl in *; auto.
+   + inv H; discriminate.
+   + exploit tr_expr_leftcontext; eauto.
+     intro. apply soundness3 in H2.
+     apply (soundness1 tmps). iIntros "HA". iDestruct (H2 with "HA") as "HA".
+     iDestruct (H3 with "HA") as (dst' sl1 sl2 a') "[P [% R]]". clear H2. clear H3.
+     simpl. iDestruct "P" as ">P". destruct dst'; norm_all.
+     * iDestruct (tr_simple_exprlist with "HG []") as "[% %]"; eauto.
+       subst; simpl. iExists _. iSplit.
+       -- iPureIntro. left. eapply plus_left. constructor.  apply star_one. econstructor; eauto.
+          eapply external_call_symbols_preserved; eauto. apply senv_preserved. traceEq.
+       -- iClear "HE HG". iConstructor. iIntros "[HB HD]".
+          iDestruct ("HD" $! (Eval vres ty) with "[]") as "HD"; eauto.
+          change sl2 with (nil ++ sl2). unfold set_opttemp.
+          iDestruct (locally_set with "[HB] HD") as "[HD HB]"; auto.
+          iApply (locally_out with "HD"). iModIntro. iSplitL "HB"; eauto.
+          iIntros. iApply locally_conseq_pure. intros. econstructor. eapply H2.
+          iApply locally_lookup. iFrame.
+     * iDestruct (tr_simple_exprlist with "HE []") as "[% %]"; eauto.
+       subst. simpl. iExists _. iSplit.
+       -- iPureIntro. left. eapply plus_left. constructor. apply star_one. econstructor; eauto.
+          eapply external_call_symbols_preserved; eauto. apply senv_preserved. traceEq.
+       -- iClear "HE". iConstructor. iIntros "HD".
+          iDestruct ("HD" $! (Eval vres ty) with "[]") as "HD"; eauto.
+          change sl2 with (nil ++ sl2). unfold set_opttemp.
+          iApply (locally_out with "HD"). iModIntro. eauto.
+     * iDestruct (tr_simple_exprlist with "HG []") as "[% %]"; eauto.
+       subst; simpl. iExists _. iSplit.
+       -- iPureIntro. left. eapply plus_left. constructor.  apply star_one. econstructor; eauto.
+          eapply external_call_symbols_preserved; eauto. apply senv_preserved. traceEq.
+       -- iClear "HG". iConstructor. iIntros "[HA [HB HD]]".
+          iDestruct ("HD" $! (Eval vres ty) with "[]") as "HD"; eauto.
+          change sl2 with (nil ++ sl2). unfold set_opttemp.
+          iDestruct (locally_set with "[HB] HD") as "[HD HB]"; auto.
+          iApply (locally_out with "HD"). iModIntro. iSplit; iFrame. iExists _. iSplitL "HB"; eauto.
+          iIntros. iApply locally_conseq_pure. intros. econstructor. eapply H2.
+          iApply locally_lookup. iFrame. eauto.
 Qed.
 
 (** Forward simulation for statements. *)
 
 Lemma tr_top_val_for_val_inv:
-  forall e le m v ty sl a tmps,
-  tr_top tge e le m For_val (Csyntax.Eval v ty) sl a tmps ->
+  forall e le m v ty sl a tmp,
+  tr_top tge e le m For_val (Csyntax.Eval v ty) sl a tmp ->
   sl = nil /\ typeof a = ty /\ eval_expr tge e le m a v.
 Proof.
-  intros. inv H. auto. inv H0. auto.
+  intros. inv H; eauto. apply (soundness1 tmp). iIntros "HA". apply soundness3 in H0.
+  iDestruct (H0 with "HA") as ">[HA [% %]]".
+  repeat iSplit; eauto. iDestruct (locally_elim with "HA") as "HA". iFrame.
 Qed.
 
 Lemma alloc_variables_preserved:
@@ -2002,28 +2176,39 @@ Proof.
   rewrite comp_env_preserved. auto.
 Qed.
 
+Lemma red_absorb : forall P tmp, (<absorb> \⌜P⌝ : iProp) () tmp -> P.
+Proof.
+  intros. apply soundness3 in H. apply (soundness1 tmp).
+  iIntros "HA". iDestruct (H with "HA") as ">$".
+Qed.
+
+Lemma red_pure : forall P tmp, (⌜P⌝ : iProp) () tmp -> P.
+Proof.
+  intros. apply soundness3 in H. apply (soundness1 tmp).
+  iIntros "HA". iDestruct (H with "HA") as "$".
+Qed.
+
 Lemma sstep_simulation:
   forall S1 t S2, Csem.sstep ge S1 t S2 ->
   forall S1' (MS: match_states S1 S1'),
   exists S2',
-     (plus step1 tge S1' t S2' \/
-       (star step1 tge S1' t S2' /\ measure S2 < measure S1)%nat)
+     (Smallstep.plus step1 tge S1' t S2' \/
+       (Smallstep.star step1 tge S1' t S2' /\ measure S2 < measure S1)%nat)
   /\ match_states S2 S2'.
 Proof.
   induction 1; intros; inv MS.
-(* do 1 *)
+  (* do 1 *)
   inv H6. inv H0.
   econstructor; split.
   right; split. apply push_seq.
-  simpl. lia.
+  simpl. unfold lt. rewrite plus_n_Sm. reflexivity.
   econstructor; eauto. constructor. auto.
-(* do 2 *)
-  inv H7. inv H6. inv H.
+  (* do 2 *)
+  inv H7. inv H6. simpl in H. apply red_absorb in H. subst.
   econstructor; split.
   right; split. apply star_refl. simpl. lia.
   econstructor; eauto. constructor.
-
-(* seq *)
+  (* seq *)
   inv H6. econstructor; split. left. apply plus_one. constructor.
   econstructor; eauto. constructor; auto.
 (* skip seq *)
@@ -2053,14 +2238,14 @@ Proof.
 (* ifthenelse *)
   inv H8.
 (* ifthenelse empty *)
-  exploit tr_top_val_for_val_inv; eauto. intros [A [B C]]. subst.
+  exploit tr_top_val_for_val_inv; eauto. intros [P0 [P1 P2]]. subst.
   econstructor; split; simpl.
   right. destruct b; econstructor; eauto.
   eapply star_left. apply step_skip_seq. econstructor. traceEq.
   eapply star_left. apply step_skip_seq. econstructor. traceEq.
   destruct b; econstructor; eauto. econstructor; eauto. econstructor; eauto.
   (* ifthenelse non empty *)
-  exploit tr_top_val_for_val_inv; eauto. intros [A [B C]]. subst.
+  exploit tr_top_val_for_val_inv; eauto. intros [P0 [P1 P2]]. subst.
   econstructor; split.
   left. eapply plus_two. constructor.
   apply step_ifthenelse with (v1 := v) (b := b); auto. traceEq.
@@ -2074,7 +2259,7 @@ Proof.
   econstructor; eauto. simpl.  econstructor; eauto. econstructor; eauto.
 (* while false *)
   inv H8.
-  exploit tr_top_val_for_val_inv; eauto. intros [A [B C]]. subst.
+  exploit tr_top_val_for_val_inv; eauto. intros [P0 [P1 P2]]. subst.
   econstructor; split.
   left. simpl. eapply plus_left. constructor.
   eapply star_trans. apply step_makeif with (v1 := v) (b := false); auto.
@@ -2083,7 +2268,7 @@ Proof.
   constructor; auto. constructor.
 (* while true *)
   inv H8.
-  exploit tr_top_val_for_val_inv; eauto. intros [A [B C]]. subst.
+  exploit tr_top_val_for_val_inv; eauto. intros [P0 [P1 P2]]. subst.
   econstructor; split.
   left. simpl. eapply plus_left. constructor.
   eapply star_right. apply step_makeif with (v1 := v) (b := true); auto.
@@ -2119,7 +2304,7 @@ Proof.
   econstructor; eauto. simpl. econstructor; auto. econstructor; eauto.
 (* dowhile false *)
   inv H8.
-  exploit tr_top_val_for_val_inv; eauto. intros [A [B C]]. subst.
+  exploit tr_top_val_for_val_inv; eauto. intros [P0 [P1 P2]]. subst.
   econstructor; split.
   left. simpl. eapply plus_left. constructor.
   eapply star_right. apply step_makeif with (v1 := v) (b := false); auto.
@@ -2128,7 +2313,7 @@ Proof.
   constructor; auto. constructor.
 (* dowhile true *)
   inv H8.
-  exploit tr_top_val_for_val_inv; eauto. intros [A [B C]]. subst.
+  exploit tr_top_val_for_val_inv; eauto. intros [P0 [P1 P2]]. subst.
   econstructor; split.
   left. simpl. eapply plus_left. constructor.
   eapply star_right. apply step_makeif with (v1 := v) (b := true); auto.
@@ -2154,7 +2339,7 @@ Proof.
   reflexivity. traceEq.
   rewrite Kseqlist_app. econstructor; eauto. simpl. constructor; auto. econstructor; eauto.
 (* for false *)
-  inv H8. exploit tr_top_val_for_val_inv; eauto. intros [A [B C]]. subst.
+  inv H8. exploit tr_top_val_for_val_inv; eauto. intros [P0 [P1 P2]]. subst.
   econstructor; split.
   left. simpl. eapply plus_left. constructor.
   eapply star_trans. apply step_makeif with (v1 := v) (b := false); auto.
@@ -2162,7 +2347,7 @@ Proof.
   reflexivity. reflexivity. traceEq.
   constructor; auto. constructor.
 (* for true *)
-  inv H8. exploit tr_top_val_for_val_inv; eauto. intros [A [B C]]. subst.
+  inv H8. exploit tr_top_val_for_val_inv; eauto. intros [P0 [P1 P2]]. subst.
   econstructor; split.
   left. simpl. eapply plus_left. constructor.
   eapply star_right. apply step_makeif with (v1 := v) (b := true); auto.
@@ -2196,7 +2381,7 @@ Proof.
   left; eapply plus_left. constructor. apply push_seq. traceEq.
   econstructor; eauto. constructor. auto.
 (* return some 2 *)
-  inv H9. exploit tr_top_val_for_val_inv; eauto. intros [A [B C]]. subst.
+  inv H9. exploit tr_top_val_for_val_inv; eauto. intros [P0 [P1 P2]]. subst.
   econstructor; split.
   left. eapply plus_two. constructor. econstructor. eauto.
   erewrite function_return_preserved; eauto. rewrite blocks_of_env_preserved; eauto.
@@ -2215,7 +2400,7 @@ Proof.
   left; eapply plus_left. constructor. apply push_seq. traceEq.
   econstructor; eauto. constructor; auto.
 (* expr switch *)
-  inv H8. exploit tr_top_val_for_val_inv; eauto. intros [A [B C]]. subst.
+  inv H8. exploit tr_top_val_for_val_inv; eauto. intros [P0 [P1 P2]]. subst.
   econstructor; split.
   left; eapply plus_two. constructor. econstructor; eauto. traceEq.
   econstructor; eauto.
@@ -2278,37 +2463,38 @@ Qed.
 
 Theorem simulation:
   forall S1 t S2, Cstrategy.step ge S1 t S2 ->
-  forall S1' (MS: match_states S1 S1'),
-  exists S2',
-     (plus step1 tge S1' t S2' \/
-       (star step1 tge S1' t S2' /\ measure S2 < measure S1)%nat)
-  /\ match_states S2 S2'.
+  forall S1', match_states S1 S1' ->
+  ∃ S2',
+     (Smallstep.plus step1 tge S1' t S2' \/
+       (Smallstep.star step1 tge S1' t S2' /\ measure S2 < measure S1)%nat)
+      /\ match_states S2 S2'.
 Proof.
   intros S1 t S2 STEP. destruct STEP.
   apply estep_simulation; auto.
   apply sstep_simulation; auto.
 Qed.
 
+
 Lemma transl_initial_states:
   forall S,
   Csem.initial_state prog S ->
-  exists S', Clight.initial_state tprog S' /\ match_states S S'.
+  exists S',  Clight.initial_state tprog S' /\ match_states S S'.
 Proof.
-  intros. inv H.
+intros. inv H.
   exploit function_ptr_translated; eauto. intros [tf [FIND TR]].
   econstructor; split.
   econstructor.
   eapply (Genv.init_mem_match (proj1 TRANSL)); eauto.
   replace (prog_main tprog) with (prog_main prog).
-  rewrite symbols_preserved. eauto. 
-  destruct TRANSL. destruct H as (A & B & C). simpl in B. auto. 
+  rewrite symbols_preserved. eauto.
+  destruct TRANSL. destruct H as (A & B & C). simpl in B. auto.
   eexact FIND.
   rewrite <- H3. apply type_of_fundef_preserved. auto.
   constructor. auto. constructor.
 Qed.
 
 Lemma transl_final_states:
-  forall S S' r,
+  ∀ S S' r,
   match_states S S' -> Csem.final_state S r -> Clight.final_state S' r.
 Proof.
   intros. inv H0. inv H. inv H4. constructor.
@@ -2331,7 +2517,7 @@ End PRESERVATION.
 
 Instance TransfSimplExprLink : TransfLink match_prog.
 Proof.
-  red; intros. eapply Ctypes.link_match_program; eauto. 
+  red; intros. eapply Ctypes.link_match_program; eauto.
 - intros.
 Local Transparent Linker_fundef.
   simpl in *; unfold link_fundef in *. inv H3; inv H4; try discriminate.
